Make round-up division always defined

dist/Klas_GEMM_Batched.cu
@@ -32,9 +32,10 @@ float
     float *out = (float *)KPR_GPU_ALLOC(4U, batch * (rows * cols));
     uint32_t idx = 0U;
     for (; idx < batch; idx++) {
+        uint32_t i = idx;
         KPR_KCALL(__hoisted_0,
-                  (rows * cols + 1023U) / 1024U,
-                  1024U, 0U, rows, shared, cols, a, b, out, idx);
+                  rows * cols / 1024U + (rows * cols % 1024U != 0U ? 1U : 0U),
+                  1024U, 0U, rows, shared, cols, a, b, out, i);
         MUST(cudaDeviceSynchronize());
     }
     return out;
