dist/Klas_GEMM_Naive2.cu
@@ -24,8 +24,9 @@ Klas_GEMM_Naive2_g_matmul_f32_rrr(uint32_t m,
                                   uint32_t n,
                                   uint32_t k, float *gA, float *gB, float *gC)
 {
-    KPR_KCALL(__hoisted_0, (m * n + 1023U) / 1024U, 1024U, 0U, m, n, k, gA, gB,
-              gC);
+    KPR_KCALL(__hoisted_0,
+              m * n / 1024U + (m * n % 1024U != 0U ? 1U : 0U),
+              1024U, 0U, m, n, k, gA, gB, gC);
     MUST(cudaDeviceSynchronize());
 }
 
@@ -53,8 +54,9 @@ Klas_GEMM_Naive2_g_matmul_f64_rrr(uint32_t m,
                                   uint32_t k,
                                   double *gA, double *gB, double *gC)
 {
-    KPR_KCALL(__hoisted_1, (m * n + 1023U) / 1024U, 1024U, 0U, m, n, k, gA, gB,
-              gC);
+    KPR_KCALL(__hoisted_1,
+              m * n / 1024U + (m * n % 1024U != 0U ? 1U : 0U),
+              1024U, 0U, m, n, k, gA, gB, gC);
     MUST(cudaDeviceSynchronize());
 }
 
@@ -83,8 +85,9 @@ Klas_GEMM_Naive2_g_matmul_u32_rrr(uint32_t m,
                                   uint32_t k,
                                   uint32_t *gA, uint32_t *gB, uint32_t *gC)
 {
-    KPR_KCALL(__hoisted_2, (m * n + 1023U) / 1024U, 1024U, 0U, m, n, k, gA, gB,
-              gC);
+    KPR_KCALL(__hoisted_2,
+              m * n / 1024U + (m * n % 1024U != 0U ? 1U : 0U),
+              1024U, 0U, m, n, k, gA, gB, gC);
     MUST(cudaDeviceSynchronize());
 }
 
@@ -113,8 +116,9 @@ Klas_GEMM_Naive2_g_matmul_u64_rrr(uint32_t m,
                                   uint32_t k,
                                   uint64_t *gA, uint64_t *gB, uint64_t *gC)
 {
-    KPR_KCALL(__hoisted_3, (m * n + 1023U) / 1024U, 1024U, 0U, m, n, k, gA, gB,
-              gC);
+    KPR_KCALL(__hoisted_3,
+              m * n / 1024U + (m * n % 1024U != 0U ? 1U : 0U),
+              1024U, 0U, m, n, k, gA, gB, gC);
     MUST(cudaDeviceSynchronize());
 }
 
@@ -141,8 +145,9 @@ Klas_GEMM_Naive2_g_matmul_f32_ccc(uint32_t m,
                                   uint32_t n,
                                   uint32_t k, float *gA, float *gB, float *gC)
 {
-    KPR_KCALL(__hoisted_4, (m * n + 1023U) / 1024U, 1024U, 0U, m, n, k, gA, gB,
-              gC);
+    KPR_KCALL(__hoisted_4,
+              m * n / 1024U + (m * n % 1024U != 0U ? 1U : 0U),
+              1024U, 0U, m, n, k, gA, gB, gC);
     MUST(cudaDeviceSynchronize());
 }
 
@@ -170,8 +175,9 @@ Klas_GEMM_Naive2_g_matmul_f64_ccc(uint32_t m,
                                   uint32_t k,
                                   double *gA, double *gB, double *gC)
 {
-    KPR_KCALL(__hoisted_5, (m * n + 1023U) / 1024U, 1024U, 0U, m, n, k, gA, gB,
-              gC);
+    KPR_KCALL(__hoisted_5,
+              m * n / 1024U + (m * n % 1024U != 0U ? 1U : 0U),
+              1024U, 0U, m, n, k, gA, gB, gC);
     MUST(cudaDeviceSynchronize());
 }
 
@@ -200,8 +206,9 @@ Klas_GEMM_Naive2_g_matmul_u32_ccc(uint32_t m,
                                   uint32_t k,
                                   uint32_t *gA, uint32_t *gB, uint32_t *gC)
 {
-    KPR_KCALL(__hoisted_6, (m * n + 1023U) / 1024U, 1024U, 0U, m, n, k, gA, gB,
-              gC);
+    KPR_KCALL(__hoisted_6,
+              m * n / 1024U + (m * n % 1024U != 0U ? 1U : 0U),
+              1024U, 0U, m, n, k, gA, gB, gC);
     MUST(cudaDeviceSynchronize());
 }
 
@@ -230,7 +237,8 @@ Klas_GEMM_Naive2_g_matmul_u64_ccc(uint32_t m,
                                   uint32_t k,
                                   uint64_t *gA, uint64_t *gB, uint64_t *gC)
 {
-    KPR_KCALL(__hoisted_7, (m * n + 1023U) / 1024U, 1024U, 0U, m, n, k, gA, gB,
-              gC);
+    KPR_KCALL(__hoisted_7,
+              m * n / 1024U + (m * n % 1024U != 0U ? 1U : 0U),
+              1024U, 0U, m, n, k, gA, gB, gC);
     MUST(cudaDeviceSynchronize());
 }
