dist/Klas_SPMM.cu
@@ -10,8 +10,10 @@ __hoisted_0(uint32_t cols,
             Kuiper_Sparse_Matrix_smatrix__uint32_t gA,
             uint32_t *row_indices, uint32_t *gB, uint32_t *gC)
 {
-    uint32_t m_idx = row_indices[blockIdx.x / ((cols + 127U) / 128U)];
-    uint32_t n_idx = blockIdx.x % ((cols + 127U) / 128U) * 128U;
+    uint32_t m_idx =
+        row_indices[blockIdx.x / (cols / 128U + (cols % 128U != 0U ? 1U : 0U))];
+    uint32_t n_idx =
+        blockIdx.x % (cols / 128U + (cols % 128U != 0U ? 1U : 0U)) * 128U;
     uint32_t *elems_tile = (uint32_t *) KPR_SHMEM_AT(0U);
     uint32_t *col_ind_tile = (uint32_t *) KPR_SHMEM_AT(512U);
     uint32_t ri = gA.row_off[m_idx];
@@ -91,8 +93,8 @@ Klas_SPMM_spmm_u32(uint32_t rows,
     KPR_SHMEM_FITS(1024U);
     MUST(cudaFuncSetAttribute
          (__hoisted_0, cudaFuncAttributeMaxDynamicSharedMemorySize, 1024U));
-    KPR_KCALL(__hoisted_0, rows * ((cols + 127U) / 128U), 32U, 1024U, cols, gA,
-              row_indices, gB, gC);
+    KPR_KCALL(__hoisted_0, rows * (cols / 128U + (cols % 128U != 0U ? 1U : 0U)),
+              32U, 1024U, cols, gA, row_indices, gB, gC);
     MUST(cudaDeviceSynchronize());
 }
 
@@ -105,8 +107,10 @@ __hoisted_1(uint32_t cols,
             Kuiper_Sparse_Matrix_smatrix__float gA,
             uint32_t *row_indices, float *gB, float *gC)
 {
-    uint32_t m_idx = row_indices[blockIdx.x / ((cols + 15U) / 16U)];
-    uint32_t n_idx = blockIdx.x % ((cols + 15U) / 16U) * 16U;
+    uint32_t m_idx =
+        row_indices[blockIdx.x / (cols / 16U + (cols % 16U != 0U ? 1U : 0U))];
+    uint32_t n_idx =
+        blockIdx.x % (cols / 16U + (cols % 16U != 0U ? 1U : 0U)) * 16U;
     float *elems_tile = (float *)KPR_SHMEM_AT(0U);
     uint32_t *col_ind_tile = (uint32_t *) KPR_SHMEM_AT(64U);
     uint32_t ri = gA.row_off[m_idx];
@@ -186,8 +190,8 @@ Klas_SPMM_g_spmm_f32_16x16x16(uint32_t rows,
     KPR_SHMEM_FITS(128U);
     MUST(cudaFuncSetAttribute
          (__hoisted_1, cudaFuncAttributeMaxDynamicSharedMemorySize, 128U));
-    KPR_KCALL(__hoisted_1, rows * ((cols + 15U) / 16U), 16U, 128U, cols, gA,
-              row_indices, gB, gC);
+    KPR_KCALL(__hoisted_1, rows * (cols / 16U + (cols % 16U != 0U ? 1U : 0U)),
+              16U, 128U, cols, gA, row_indices, gB, gC);
     MUST(cudaDeviceSynchronize());
 }
 
@@ -200,8 +204,10 @@ __hoisted_2(uint32_t cols,
             Kuiper_Sparse_Matrix_smatrix__float gA,
             uint32_t *row_indices, float *gB, float *gC)
 {
-    uint32_t m_idx = row_indices[blockIdx.x / ((cols + 15U) / 16U)];
-    uint32_t n_idx = blockIdx.x % ((cols + 15U) / 16U) * 16U;
+    uint32_t m_idx =
+        row_indices[blockIdx.x / (cols / 16U + (cols % 16U != 0U ? 1U : 0U))];
+    uint32_t n_idx =
+        blockIdx.x % (cols / 16U + (cols % 16U != 0U ? 1U : 0U)) * 16U;
     float *elems_tile = (float *)KPR_SHMEM_AT(0U);
     uint32_t *col_ind_tile = (uint32_t *) KPR_SHMEM_AT(128U);
     uint32_t ri = gA.row_off[m_idx];
@@ -281,8 +287,8 @@ Klas_SPMM_g_spmm_f32_16x32x16(uint32_t rows,
     KPR_SHMEM_FITS(256U);
     MUST(cudaFuncSetAttribute
          (__hoisted_2, cudaFuncAttributeMaxDynamicSharedMemorySize, 256U));
-    KPR_KCALL(__hoisted_2, rows * ((cols + 15U) / 16U), 16U, 256U, cols, gA,
-              row_indices, gB, gC);
+    KPR_KCALL(__hoisted_2, rows * (cols / 16U + (cols % 16U != 0U ? 1U : 0U)),
+              16U, 256U, cols, gA, row_indices, gB, gC);
     MUST(cudaDeviceSynchronize());
 }
 
@@ -295,8 +301,10 @@ __hoisted_3(uint32_t cols,
             Kuiper_Sparse_Matrix_smatrix__float gA,
             uint32_t *row_indices, float *gB, float *gC)
 {
-    uint32_t m_idx = row_indices[blockIdx.x / ((cols + 15U) / 16U)];
-    uint32_t n_idx = blockIdx.x % ((cols + 15U) / 16U) * 16U;
+    uint32_t m_idx =
+        row_indices[blockIdx.x / (cols / 16U + (cols % 16U != 0U ? 1U : 0U))];
+    uint32_t n_idx =
+        blockIdx.x % (cols / 16U + (cols % 16U != 0U ? 1U : 0U)) * 16U;
     float *elems_tile = (float *)KPR_SHMEM_AT(0U);
     uint32_t *col_ind_tile = (uint32_t *) KPR_SHMEM_AT(256U);
     uint32_t ri = gA.row_off[m_idx];
@@ -376,8 +384,8 @@ Klas_SPMM_g_spmm_f32_16x64x16(uint32_t rows,
     KPR_SHMEM_FITS(512U);
     MUST(cudaFuncSetAttribute
          (__hoisted_3, cudaFuncAttributeMaxDynamicSharedMemorySize, 512U));
-    KPR_KCALL(__hoisted_3, rows * ((cols + 15U) / 16U), 16U, 512U, cols, gA,
-              row_indices, gB, gC);
+    KPR_KCALL(__hoisted_3, rows * (cols / 16U + (cols % 16U != 0U ? 1U : 0U)),
+              16U, 512U, cols, gA, row_indices, gB, gC);
     MUST(cudaDeviceSynchronize());
 }
 
@@ -390,8 +398,10 @@ __hoisted_4(uint32_t cols,
             Kuiper_Sparse_Matrix_smatrix__float gA,
             uint32_t *row_indices, float *gB, float *gC)
 {
-    uint32_t m_idx = row_indices[blockIdx.x / ((cols + 15U) / 16U)];
-    uint32_t n_idx = blockIdx.x % ((cols + 15U) / 16U) * 16U;
+    uint32_t m_idx =
+        row_indices[blockIdx.x / (cols / 16U + (cols % 16U != 0U ? 1U : 0U))];
+    uint32_t n_idx =
+        blockIdx.x % (cols / 16U + (cols % 16U != 0U ? 1U : 0U)) * 16U;
     float *elems_tile = (float *)KPR_SHMEM_AT(0U);
     uint32_t *col_ind_tile = (uint32_t *) KPR_SHMEM_AT(512U);
     uint32_t ri = gA.row_off[m_idx];
@@ -471,8 +481,8 @@ Klas_SPMM_g_spmm_f32_16x128x16(uint32_t rows,
     KPR_SHMEM_FITS(1024U);
     MUST(cudaFuncSetAttribute
          (__hoisted_4, cudaFuncAttributeMaxDynamicSharedMemorySize, 1024U));
-    KPR_KCALL(__hoisted_4, rows * ((cols + 15U) / 16U), 16U, 1024U, cols, gA,
-              row_indices, gB, gC);
+    KPR_KCALL(__hoisted_4, rows * (cols / 16U + (cols % 16U != 0U ? 1U : 0U)),
+              16U, 1024U, cols, gA, row_indices, gB, gC);
     MUST(cudaDeviceSynchronize());
 }
 
@@ -485,8 +495,10 @@ __hoisted_5(uint32_t cols,
             Kuiper_Sparse_Matrix_smatrix__float gA,
             uint32_t *row_indices, float *gB, float *gC)
 {
-    uint32_t m_idx = row_indices[blockIdx.x / ((cols + 15U) / 16U)];
-    uint32_t n_idx = blockIdx.x % ((cols + 15U) / 16U) * 16U;
+    uint32_t m_idx =
+        row_indices[blockIdx.x / (cols / 16U + (cols % 16U != 0U ? 1U : 0U))];
+    uint32_t n_idx =
+        blockIdx.x % (cols / 16U + (cols % 16U != 0U ? 1U : 0U)) * 16U;
     float *elems_tile = (float *)KPR_SHMEM_AT(0U);
     uint32_t *col_ind_tile = (uint32_t *) KPR_SHMEM_AT(1024U);
     uint32_t ri = gA.row_off[m_idx];
@@ -566,8 +578,8 @@ Klas_SPMM_g_spmm_f32_16x256x16(uint32_t rows,
     KPR_SHMEM_FITS(2048U);
     MUST(cudaFuncSetAttribute
          (__hoisted_5, cudaFuncAttributeMaxDynamicSharedMemorySize, 2048U));
-    KPR_KCALL(__hoisted_5, rows * ((cols + 15U) / 16U), 16U, 2048U, cols, gA,
-              row_indices, gB, gC);
+    KPR_KCALL(__hoisted_5, rows * (cols / 16U + (cols % 16U != 0U ? 1U : 0U)),
+              16U, 2048U, cols, gA, row_indices, gB, gC);
     MUST(cudaDeviceSynchronize());
 }
 
@@ -580,8 +592,10 @@ __hoisted_6(uint32_t cols,
             Kuiper_Sparse_Matrix_smatrix__float gA,
             uint32_t *row_indices, float *gB, float *gC)
 {
-    uint32_t m_idx = row_indices[blockIdx.x / ((cols + 15U) / 16U)];
-    uint32_t n_idx = blockIdx.x % ((cols + 15U) / 16U) * 16U;
+    uint32_t m_idx =
+        row_indices[blockIdx.x / (cols / 16U + (cols % 16U != 0U ? 1U : 0U))];
+    uint32_t n_idx =
+        blockIdx.x % (cols / 16U + (cols % 16U != 0U ? 1U : 0U)) * 16U;
     float *elems_tile = (float *)KPR_SHMEM_AT(0U);
     uint32_t *col_ind_tile = (uint32_t *) KPR_SHMEM_AT(2048U);
     uint32_t ri = gA.row_off[m_idx];
@@ -661,8 +675,8 @@ Klas_SPMM_g_spmm_f32_16x512x16(uint32_t rows,
     KPR_SHMEM_FITS(4096U);
     MUST(cudaFuncSetAttribute
          (__hoisted_6, cudaFuncAttributeMaxDynamicSharedMemorySize, 4096U));
-    KPR_KCALL(__hoisted_6, rows * ((cols + 15U) / 16U), 16U, 4096U, cols, gA,
-              row_indices, gB, gC);
+    KPR_KCALL(__hoisted_6, rows * (cols / 16U + (cols % 16U != 0U ? 1U : 0U)),
+              16U, 4096U, cols, gA, row_indices, gB, gC);
     MUST(cudaDeviceSynchronize());
 }
 
@@ -675,8 +689,10 @@ __hoisted_7(uint32_t cols,
             Kuiper_Sparse_Matrix_smatrix__float gA,
             uint32_t *row_indices, float *gB, float *gC)
 {
-    uint32_t m_idx = row_indices[blockIdx.x / ((cols + 31U) / 32U)];
-    uint32_t n_idx = blockIdx.x % ((cols + 31U) / 32U) * 32U;
+    uint32_t m_idx =
+        row_indices[blockIdx.x / (cols / 32U + (cols % 32U != 0U ? 1U : 0U))];
+    uint32_t n_idx =
+        blockIdx.x % (cols / 32U + (cols % 32U != 0U ? 1U : 0U)) * 32U;
     float *elems_tile = (float *)KPR_SHMEM_AT(0U);
     uint32_t *col_ind_tile = (uint32_t *) KPR_SHMEM_AT(64U);
     uint32_t ri = gA.row_off[m_idx];
@@ -757,8 +773,8 @@ Klas_SPMM_g_spmm_f32_32x16x16(uint32_t rows,
     KPR_SHMEM_FITS(128U);
     MUST(cudaFuncSetAttribute
          (__hoisted_7, cudaFuncAttributeMaxDynamicSharedMemorySize, 128U));
-    KPR_KCALL(__hoisted_7, rows * ((cols + 31U) / 32U), 16U, 128U, cols, gA,
-              row_indices, gB, gC);
+    KPR_KCALL(__hoisted_7, rows * (cols / 32U + (cols % 32U != 0U ? 1U : 0U)),
+              16U, 128U, cols, gA, row_indices, gB, gC);
     MUST(cudaDeviceSynchronize());
 }
 
@@ -771,8 +787,10 @@ __hoisted_8(uint32_t cols,
             Kuiper_Sparse_Matrix_smatrix__float gA,
             uint32_t *row_indices, float *gB, float *gC)
 {
-    uint32_t m_idx = row_indices[blockIdx.x / ((cols + 31U) / 32U)];
-    uint32_t n_idx = blockIdx.x % ((cols + 31U) / 32U) * 32U;
+    uint32_t m_idx =
+        row_indices[blockIdx.x / (cols / 32U + (cols % 32U != 0U ? 1U : 0U))];
+    uint32_t n_idx =
+        blockIdx.x % (cols / 32U + (cols % 32U != 0U ? 1U : 0U)) * 32U;
     float *elems_tile = (float *)KPR_SHMEM_AT(0U);
     uint32_t *col_ind_tile = (uint32_t *) KPR_SHMEM_AT(128U);
     uint32_t ri = gA.row_off[m_idx];
@@ -853,8 +871,8 @@ Klas_SPMM_g_spmm_f32_32x32x16(uint32_t rows,
     KPR_SHMEM_FITS(256U);
     MUST(cudaFuncSetAttribute
          (__hoisted_8, cudaFuncAttributeMaxDynamicSharedMemorySize, 256U));
-    KPR_KCALL(__hoisted_8, rows * ((cols + 31U) / 32U), 16U, 256U, cols, gA,
-              row_indices, gB, gC);
+    KPR_KCALL(__hoisted_8, rows * (cols / 32U + (cols % 32U != 0U ? 1U : 0U)),
+              16U, 256U, cols, gA, row_indices, gB, gC);
     MUST(cudaDeviceSynchronize());
 }
 
@@ -867,8 +885,10 @@ __hoisted_9(uint32_t cols,
             Kuiper_Sparse_Matrix_smatrix__float gA,
             uint32_t *row_indices, float *gB, float *gC)
 {
-    uint32_t m_idx = row_indices[blockIdx.x / ((cols + 31U) / 32U)];
-    uint32_t n_idx = blockIdx.x % ((cols + 31U) / 32U) * 32U;
+    uint32_t m_idx =
+        row_indices[blockIdx.x / (cols / 32U + (cols % 32U != 0U ? 1U : 0U))];
+    uint32_t n_idx =
+        blockIdx.x % (cols / 32U + (cols % 32U != 0U ? 1U : 0U)) * 32U;
     float *elems_tile = (float *)KPR_SHMEM_AT(0U);
     uint32_t *col_ind_tile = (uint32_t *) KPR_SHMEM_AT(128U);
     uint32_t ri = gA.row_off[m_idx];
@@ -948,8 +968,8 @@ Klas_SPMM_g_spmm_f32_32x32x32(uint32_t rows,
     KPR_SHMEM_FITS(256U);
     MUST(cudaFuncSetAttribute
          (__hoisted_9, cudaFuncAttributeMaxDynamicSharedMemorySize, 256U));
-    KPR_KCALL(__hoisted_9, rows * ((cols + 31U) / 32U), 32U, 256U, cols, gA,
-              row_indices, gB, gC);
+    KPR_KCALL(__hoisted_9, rows * (cols / 32U + (cols % 32U != 0U ? 1U : 0U)),
+              32U, 256U, cols, gA, row_indices, gB, gC);
     MUST(cudaDeviceSynchronize());
 }
 
@@ -962,8 +982,10 @@ __hoisted_10(uint32_t cols,
              Kuiper_Sparse_Matrix_smatrix__float gA,
              uint32_t *row_indices, float *gB, float *gC)
 {
-    uint32_t m_idx = row_indices[blockIdx.x / ((cols + 31U) / 32U)];
-    uint32_t n_idx = blockIdx.x % ((cols + 31U) / 32U) * 32U;
+    uint32_t m_idx =
+        row_indices[blockIdx.x / (cols / 32U + (cols % 32U != 0U ? 1U : 0U))];
+    uint32_t n_idx =
+        blockIdx.x % (cols / 32U + (cols % 32U != 0U ? 1U : 0U)) * 32U;
     float *elems_tile = (float *)KPR_SHMEM_AT(0U);
     uint32_t *col_ind_tile = (uint32_t *) KPR_SHMEM_AT(256U);
     uint32_t ri = gA.row_off[m_idx];
@@ -1044,8 +1066,8 @@ Klas_SPMM_g_spmm_f32_32x64x16(uint32_t rows,
     KPR_SHMEM_FITS(512U);
     MUST(cudaFuncSetAttribute
          (__hoisted_10, cudaFuncAttributeMaxDynamicSharedMemorySize, 512U));
-    KPR_KCALL(__hoisted_10, rows * ((cols + 31U) / 32U), 16U, 512U, cols, gA,
-              row_indices, gB, gC);
+    KPR_KCALL(__hoisted_10, rows * (cols / 32U + (cols % 32U != 0U ? 1U : 0U)),
+              16U, 512U, cols, gA, row_indices, gB, gC);
     MUST(cudaDeviceSynchronize());
 }
 
@@ -1058,8 +1080,10 @@ __hoisted_11(uint32_t cols,
              Kuiper_Sparse_Matrix_smatrix__float gA,
              uint32_t *row_indices, float *gB, float *gC)
 {
-    uint32_t m_idx = row_indices[blockIdx.x / ((cols + 31U) / 32U)];
-    uint32_t n_idx = blockIdx.x % ((cols + 31U) / 32U) * 32U;
+    uint32_t m_idx =
+        row_indices[blockIdx.x / (cols / 32U + (cols % 32U != 0U ? 1U : 0U))];
+    uint32_t n_idx =
+        blockIdx.x % (cols / 32U + (cols % 32U != 0U ? 1U : 0U)) * 32U;
     float *elems_tile = (float *)KPR_SHMEM_AT(0U);
     uint32_t *col_ind_tile = (uint32_t *) KPR_SHMEM_AT(256U);
     uint32_t ri = gA.row_off[m_idx];
@@ -1139,8 +1163,8 @@ Klas_SPMM_g_spmm_f32_32x64x32(uint32_t rows,
     KPR_SHMEM_FITS(512U);
     MUST(cudaFuncSetAttribute
          (__hoisted_11, cudaFuncAttributeMaxDynamicSharedMemorySize, 512U));
-    KPR_KCALL(__hoisted_11, rows * ((cols + 31U) / 32U), 32U, 512U, cols, gA,
-              row_indices, gB, gC);
+    KPR_KCALL(__hoisted_11, rows * (cols / 32U + (cols % 32U != 0U ? 1U : 0U)),
+              32U, 512U, cols, gA, row_indices, gB, gC);
     MUST(cudaDeviceSynchronize());
 }
 
@@ -1153,8 +1177,10 @@ __hoisted_12(uint32_t cols,
              Kuiper_Sparse_Matrix_smatrix__float gA,
              uint32_t *row_indices, float *gB, float *gC)
 {
-    uint32_t m_idx = row_indices[blockIdx.x / ((cols + 31U) / 32U)];
-    uint32_t n_idx = blockIdx.x % ((cols + 31U) / 32U) * 32U;
+    uint32_t m_idx =
+        row_indices[blockIdx.x / (cols / 32U + (cols % 32U != 0U ? 1U : 0U))];
+    uint32_t n_idx =
+        blockIdx.x % (cols / 32U + (cols % 32U != 0U ? 1U : 0U)) * 32U;
     float *elems_tile = (float *)KPR_SHMEM_AT(0U);
     uint32_t *col_ind_tile = (uint32_t *) KPR_SHMEM_AT(512U);
     uint32_t ri = gA.row_off[m_idx];
@@ -1235,8 +1261,8 @@ Klas_SPMM_g_spmm_f32_32x128x16(uint32_t rows,
     KPR_SHMEM_FITS(1024U);
     MUST(cudaFuncSetAttribute
          (__hoisted_12, cudaFuncAttributeMaxDynamicSharedMemorySize, 1024U));
-    KPR_KCALL(__hoisted_12, rows * ((cols + 31U) / 32U), 16U, 1024U, cols, gA,
-              row_indices, gB, gC);
+    KPR_KCALL(__hoisted_12, rows * (cols / 32U + (cols % 32U != 0U ? 1U : 0U)),
+              16U, 1024U, cols, gA, row_indices, gB, gC);
     MUST(cudaDeviceSynchronize());
 }
 
@@ -1249,8 +1275,10 @@ __hoisted_13(uint32_t cols,
              Kuiper_Sparse_Matrix_smatrix__float gA,
              uint32_t *row_indices, float *gB, float *gC)
 {
-    uint32_t m_idx = row_indices[blockIdx.x / ((cols + 31U) / 32U)];
-    uint32_t n_idx = blockIdx.x % ((cols + 31U) / 32U) * 32U;
+    uint32_t m_idx =
+        row_indices[blockIdx.x / (cols / 32U + (cols % 32U != 0U ? 1U : 0U))];
+    uint32_t n_idx =
+        blockIdx.x % (cols / 32U + (cols % 32U != 0U ? 1U : 0U)) * 32U;
     float *elems_tile = (float *)KPR_SHMEM_AT(0U);
     uint32_t *col_ind_tile = (uint32_t *) KPR_SHMEM_AT(512U);
     uint32_t ri = gA.row_off[m_idx];
@@ -1330,8 +1358,8 @@ Klas_SPMM_g_spmm_f32_32x128x32(uint32_t rows,
     KPR_SHMEM_FITS(1024U);
     MUST(cudaFuncSetAttribute
          (__hoisted_13, cudaFuncAttributeMaxDynamicSharedMemorySize, 1024U));
-    KPR_KCALL(__hoisted_13, rows * ((cols + 31U) / 32U), 32U, 1024U, cols, gA,
-              row_indices, gB, gC);
+    KPR_KCALL(__hoisted_13, rows * (cols / 32U + (cols % 32U != 0U ? 1U : 0U)),
+              32U, 1024U, cols, gA, row_indices, gB, gC);
     MUST(cudaDeviceSynchronize());
 }
 
@@ -1344,8 +1372,10 @@ __hoisted_14(uint32_t cols,
              Kuiper_Sparse_Matrix_smatrix__float gA,
              uint32_t *row_indices, float *gB, float *gC)
 {
-    uint32_t m_idx = row_indices[blockIdx.x / ((cols + 31U) / 32U)];
-    uint32_t n_idx = blockIdx.x % ((cols + 31U) / 32U) * 32U;
+    uint32_t m_idx =
+        row_indices[blockIdx.x / (cols / 32U + (cols % 32U != 0U ? 1U : 0U))];
+    uint32_t n_idx =
+        blockIdx.x % (cols / 32U + (cols % 32U != 0U ? 1U : 0U)) * 32U;
     float *elems_tile = (float *)KPR_SHMEM_AT(0U);
     uint32_t *col_ind_tile = (uint32_t *) KPR_SHMEM_AT(1024U);
     uint32_t ri = gA.row_off[m_idx];
@@ -1426,8 +1456,8 @@ Klas_SPMM_g_spmm_f32_32x256x16(uint32_t rows,
     KPR_SHMEM_FITS(2048U);
     MUST(cudaFuncSetAttribute
          (__hoisted_14, cudaFuncAttributeMaxDynamicSharedMemorySize, 2048U));
-    KPR_KCALL(__hoisted_14, rows * ((cols + 31U) / 32U), 16U, 2048U, cols, gA,
-              row_indices, gB, gC);
+    KPR_KCALL(__hoisted_14, rows * (cols / 32U + (cols % 32U != 0U ? 1U : 0U)),
+              16U, 2048U, cols, gA, row_indices, gB, gC);
     MUST(cudaDeviceSynchronize());
 }
 
@@ -1440,8 +1470,10 @@ __hoisted_15(uint32_t cols,
              Kuiper_Sparse_Matrix_smatrix__float gA,
              uint32_t *row_indices, float *gB, float *gC)
 {
-    uint32_t m_idx = row_indices[blockIdx.x / ((cols + 31U) / 32U)];
-    uint32_t n_idx = blockIdx.x % ((cols + 31U) / 32U) * 32U;
+    uint32_t m_idx =
+        row_indices[blockIdx.x / (cols / 32U + (cols % 32U != 0U ? 1U : 0U))];
+    uint32_t n_idx =
+        blockIdx.x % (cols / 32U + (cols % 32U != 0U ? 1U : 0U)) * 32U;
     float *elems_tile = (float *)KPR_SHMEM_AT(0U);
     uint32_t *col_ind_tile = (uint32_t *) KPR_SHMEM_AT(1024U);
     uint32_t ri = gA.row_off[m_idx];
@@ -1521,8 +1553,8 @@ Klas_SPMM_g_spmm_f32_32x256x32(uint32_t rows,
     KPR_SHMEM_FITS(2048U);
     MUST(cudaFuncSetAttribute
          (__hoisted_15, cudaFuncAttributeMaxDynamicSharedMemorySize, 2048U));
-    KPR_KCALL(__hoisted_15, rows * ((cols + 31U) / 32U), 32U, 2048U, cols, gA,
-              row_indices, gB, gC);
+    KPR_KCALL(__hoisted_15, rows * (cols / 32U + (cols % 32U != 0U ? 1U : 0U)),
+              32U, 2048U, cols, gA, row_indices, gB, gC);
     MUST(cudaDeviceSynchronize());
 }
 
@@ -1535,8 +1567,10 @@ __hoisted_16(uint32_t cols,
              Kuiper_Sparse_Matrix_smatrix__float gA,
              uint32_t *row_indices, float *gB, float *gC)
 {
-    uint32_t m_idx = row_indices[blockIdx.x / ((cols + 31U) / 32U)];
-    uint32_t n_idx = blockIdx.x % ((cols + 31U) / 32U) * 32U;
+    uint32_t m_idx =
+        row_indices[blockIdx.x / (cols / 32U + (cols % 32U != 0U ? 1U : 0U))];
+    uint32_t n_idx =
+        blockIdx.x % (cols / 32U + (cols % 32U != 0U ? 1U : 0U)) * 32U;
     float *elems_tile = (float *)KPR_SHMEM_AT(0U);
     uint32_t *col_ind_tile = (uint32_t *) KPR_SHMEM_AT(2048U);
     uint32_t ri = gA.row_off[m_idx];
@@ -1617,8 +1651,8 @@ Klas_SPMM_g_spmm_f32_32x512x16(uint32_t rows,
     KPR_SHMEM_FITS(4096U);
     MUST(cudaFuncSetAttribute
          (__hoisted_16, cudaFuncAttributeMaxDynamicSharedMemorySize, 4096U));
-    KPR_KCALL(__hoisted_16, rows * ((cols + 31U) / 32U), 16U, 4096U, cols, gA,
-              row_indices, gB, gC);
+    KPR_KCALL(__hoisted_16, rows * (cols / 32U + (cols % 32U != 0U ? 1U : 0U)),
+              16U, 4096U, cols, gA, row_indices, gB, gC);
     MUST(cudaDeviceSynchronize());
 }
 
@@ -1631,8 +1665,10 @@ __hoisted_17(uint32_t cols,
              Kuiper_Sparse_Matrix_smatrix__float gA,
              uint32_t *row_indices, float *gB, float *gC)
 {
-    uint32_t m_idx = row_indices[blockIdx.x / ((cols + 31U) / 32U)];
-    uint32_t n_idx = blockIdx.x % ((cols + 31U) / 32U) * 32U;
+    uint32_t m_idx =
+        row_indices[blockIdx.x / (cols / 32U + (cols % 32U != 0U ? 1U : 0U))];
+    uint32_t n_idx =
+        blockIdx.x % (cols / 32U + (cols % 32U != 0U ? 1U : 0U)) * 32U;
     float *elems_tile = (float *)KPR_SHMEM_AT(0U);
     uint32_t *col_ind_tile = (uint32_t *) KPR_SHMEM_AT(2048U);
     uint32_t ri = gA.row_off[m_idx];
@@ -1712,8 +1748,8 @@ Klas_SPMM_g_spmm_f32_32x512x32(uint32_t rows,
     KPR_SHMEM_FITS(4096U);
     MUST(cudaFuncSetAttribute
          (__hoisted_17, cudaFuncAttributeMaxDynamicSharedMemorySize, 4096U));
-    KPR_KCALL(__hoisted_17, rows * ((cols + 31U) / 32U), 32U, 4096U, cols, gA,
-              row_indices, gB, gC);
+    KPR_KCALL(__hoisted_17, rows * (cols / 32U + (cols % 32U != 0U ? 1U : 0U)),
+              32U, 4096U, cols, gA, row_indices, gB, gC);
     MUST(cudaDeviceSynchronize());
 }
 
@@ -1726,8 +1762,10 @@ __hoisted_18(uint32_t cols,
              Kuiper_Sparse_Matrix_smatrix__float gA,
              uint32_t *row_indices, float *gB, float *gC)
 {
-    uint32_t m_idx = row_indices[blockIdx.x / ((cols + 63U) / 64U)];
-    uint32_t n_idx = blockIdx.x % ((cols + 63U) / 64U) * 64U;
+    uint32_t m_idx =
+        row_indices[blockIdx.x / (cols / 64U + (cols % 64U != 0U ? 1U : 0U))];
+    uint32_t n_idx =
+        blockIdx.x % (cols / 64U + (cols % 64U != 0U ? 1U : 0U)) * 64U;
     float *elems_tile = (float *)KPR_SHMEM_AT(0U);
     uint32_t *col_ind_tile = (uint32_t *) KPR_SHMEM_AT(64U);
     uint32_t ri = gA.row_off[m_idx];
@@ -1808,8 +1846,8 @@ Klas_SPMM_g_spmm_f32_64x16x16(uint32_t rows,
     KPR_SHMEM_FITS(128U);
     MUST(cudaFuncSetAttribute
          (__hoisted_18, cudaFuncAttributeMaxDynamicSharedMemorySize, 128U));
-    KPR_KCALL(__hoisted_18, rows * ((cols + 63U) / 64U), 16U, 128U, cols, gA,
-              row_indices, gB, gC);
+    KPR_KCALL(__hoisted_18, rows * (cols / 64U + (cols % 64U != 0U ? 1U : 0U)),
+              16U, 128U, cols, gA, row_indices, gB, gC);
     MUST(cudaDeviceSynchronize());
 }
 
@@ -1822,8 +1860,10 @@ __hoisted_19(uint32_t cols,
              Kuiper_Sparse_Matrix_smatrix__float gA,
              uint32_t *row_indices, float *gB, float *gC)
 {
-    uint32_t m_idx = row_indices[blockIdx.x / ((cols + 63U) / 64U)];
-    uint32_t n_idx = blockIdx.x % ((cols + 63U) / 64U) * 64U;
+    uint32_t m_idx =
+        row_indices[blockIdx.x / (cols / 64U + (cols % 64U != 0U ? 1U : 0U))];
+    uint32_t n_idx =
+        blockIdx.x % (cols / 64U + (cols % 64U != 0U ? 1U : 0U)) * 64U;
     float *elems_tile = (float *)KPR_SHMEM_AT(0U);
     uint32_t *col_ind_tile = (uint32_t *) KPR_SHMEM_AT(128U);
     uint32_t ri = gA.row_off[m_idx];
@@ -1904,8 +1944,8 @@ Klas_SPMM_g_spmm_f32_64x32x16(uint32_t rows,
     KPR_SHMEM_FITS(256U);
     MUST(cudaFuncSetAttribute
          (__hoisted_19, cudaFuncAttributeMaxDynamicSharedMemorySize, 256U));
-    KPR_KCALL(__hoisted_19, rows * ((cols + 63U) / 64U), 16U, 256U, cols, gA,
-              row_indices, gB, gC);
+    KPR_KCALL(__hoisted_19, rows * (cols / 64U + (cols % 64U != 0U ? 1U : 0U)),
+              16U, 256U, cols, gA, row_indices, gB, gC);
     MUST(cudaDeviceSynchronize());
 }
 
@@ -1918,8 +1958,10 @@ __hoisted_20(uint32_t cols,
              Kuiper_Sparse_Matrix_smatrix__float gA,
              uint32_t *row_indices, float *gB, float *gC)
 {
-    uint32_t m_idx = row_indices[blockIdx.x / ((cols + 63U) / 64U)];
-    uint32_t n_idx = blockIdx.x % ((cols + 63U) / 64U) * 64U;
+    uint32_t m_idx =
+        row_indices[blockIdx.x / (cols / 64U + (cols % 64U != 0U ? 1U : 0U))];
+    uint32_t n_idx =
+        blockIdx.x % (cols / 64U + (cols % 64U != 0U ? 1U : 0U)) * 64U;
     float *elems_tile = (float *)KPR_SHMEM_AT(0U);
     uint32_t *col_ind_tile = (uint32_t *) KPR_SHMEM_AT(128U);
     uint32_t ri = gA.row_off[m_idx];
@@ -2000,8 +2042,8 @@ Klas_SPMM_g_spmm_f32_64x32x32(uint32_t rows,
     KPR_SHMEM_FITS(256U);
     MUST(cudaFuncSetAttribute
          (__hoisted_20, cudaFuncAttributeMaxDynamicSharedMemorySize, 256U));
-    KPR_KCALL(__hoisted_20, rows * ((cols + 63U) / 64U), 32U, 256U, cols, gA,
-              row_indices, gB, gC);
+    KPR_KCALL(__hoisted_20, rows * (cols / 64U + (cols % 64U != 0U ? 1U : 0U)),
+              32U, 256U, cols, gA, row_indices, gB, gC);
     MUST(cudaDeviceSynchronize());
 }
 
@@ -2014,8 +2056,10 @@ __hoisted_21(uint32_t cols,
              Kuiper_Sparse_Matrix_smatrix__float gA,
              uint32_t *row_indices, float *gB, float *gC)
 {
-    uint32_t m_idx = row_indices[blockIdx.x / ((cols + 63U) / 64U)];
-    uint32_t n_idx = blockIdx.x % ((cols + 63U) / 64U) * 64U;
+    uint32_t m_idx =
+        row_indices[blockIdx.x / (cols / 64U + (cols % 64U != 0U ? 1U : 0U))];
+    uint32_t n_idx =
+        blockIdx.x % (cols / 64U + (cols % 64U != 0U ? 1U : 0U)) * 64U;
     float *elems_tile = (float *)KPR_SHMEM_AT(0U);
     uint32_t *col_ind_tile = (uint32_t *) KPR_SHMEM_AT(256U);
     uint32_t ri = gA.row_off[m_idx];
@@ -2096,8 +2140,8 @@ Klas_SPMM_g_spmm_f32_64x64x16(uint32_t rows,
     KPR_SHMEM_FITS(512U);
     MUST(cudaFuncSetAttribute
          (__hoisted_21, cudaFuncAttributeMaxDynamicSharedMemorySize, 512U));
-    KPR_KCALL(__hoisted_21, rows * ((cols + 63U) / 64U), 16U, 512U, cols, gA,
-              row_indices, gB, gC);
+    KPR_KCALL(__hoisted_21, rows * (cols / 64U + (cols % 64U != 0U ? 1U : 0U)),
+              16U, 512U, cols, gA, row_indices, gB, gC);
     MUST(cudaDeviceSynchronize());
 }
 
@@ -2110,8 +2154,10 @@ __hoisted_22(uint32_t cols,
              Kuiper_Sparse_Matrix_smatrix__float gA,
              uint32_t *row_indices, float *gB, float *gC)
 {
-    uint32_t m_idx = row_indices[blockIdx.x / ((cols + 63U) / 64U)];
-    uint32_t n_idx = blockIdx.x % ((cols + 63U) / 64U) * 64U;
+    uint32_t m_idx =
+        row_indices[blockIdx.x / (cols / 64U + (cols % 64U != 0U ? 1U : 0U))];
+    uint32_t n_idx =
+        blockIdx.x % (cols / 64U + (cols % 64U != 0U ? 1U : 0U)) * 64U;
     float *elems_tile = (float *)KPR_SHMEM_AT(0U);
     uint32_t *col_ind_tile = (uint32_t *) KPR_SHMEM_AT(256U);
     uint32_t ri = gA.row_off[m_idx];
@@ -2192,8 +2238,8 @@ Klas_SPMM_g_spmm_f32_64x64x32(uint32_t rows,
     KPR_SHMEM_FITS(512U);
     MUST(cudaFuncSetAttribute
          (__hoisted_22, cudaFuncAttributeMaxDynamicSharedMemorySize, 512U));
-    KPR_KCALL(__hoisted_22, rows * ((cols + 63U) / 64U), 32U, 512U, cols, gA,
-              row_indices, gB, gC);
+    KPR_KCALL(__hoisted_22, rows * (cols / 64U + (cols % 64U != 0U ? 1U : 0U)),
+              32U, 512U, cols, gA, row_indices, gB, gC);
     MUST(cudaDeviceSynchronize());
 }
 
@@ -2206,8 +2252,10 @@ __hoisted_23(uint32_t cols,
              Kuiper_Sparse_Matrix_smatrix__float gA,
              uint32_t *row_indices, float *gB, float *gC)
 {
-    uint32_t m_idx = row_indices[blockIdx.x / ((cols + 63U) / 64U)];
-    uint32_t n_idx = blockIdx.x % ((cols + 63U) / 64U) * 64U;
+    uint32_t m_idx =
+        row_indices[blockIdx.x / (cols / 64U + (cols % 64U != 0U ? 1U : 0U))];
+    uint32_t n_idx =
+        blockIdx.x % (cols / 64U + (cols % 64U != 0U ? 1U : 0U)) * 64U;
     float *elems_tile = (float *)KPR_SHMEM_AT(0U);
     uint32_t *col_ind_tile = (uint32_t *) KPR_SHMEM_AT(256U);
     uint32_t ri = gA.row_off[m_idx];
@@ -2287,8 +2335,8 @@ Klas_SPMM_g_spmm_f32_64x64x64(uint32_t rows,
     KPR_SHMEM_FITS(512U);
     MUST(cudaFuncSetAttribute
          (__hoisted_23, cudaFuncAttributeMaxDynamicSharedMemorySize, 512U));
-    KPR_KCALL(__hoisted_23, rows * ((cols + 63U) / 64U), 64U, 512U, cols, gA,
-              row_indices, gB, gC);
+    KPR_KCALL(__hoisted_23, rows * (cols / 64U + (cols % 64U != 0U ? 1U : 0U)),
+              64U, 512U, cols, gA, row_indices, gB, gC);
     MUST(cudaDeviceSynchronize());
 }
 
@@ -2301,8 +2349,10 @@ __hoisted_24(uint32_t cols,
              Kuiper_Sparse_Matrix_smatrix__float gA,
              uint32_t *row_indices, float *gB, float *gC)
 {
-    uint32_t m_idx = row_indices[blockIdx.x / ((cols + 63U) / 64U)];
-    uint32_t n_idx = blockIdx.x % ((cols + 63U) / 64U) * 64U;
+    uint32_t m_idx =
+        row_indices[blockIdx.x / (cols / 64U + (cols % 64U != 0U ? 1U : 0U))];
+    uint32_t n_idx =
+        blockIdx.x % (cols / 64U + (cols % 64U != 0U ? 1U : 0U)) * 64U;
     float *elems_tile = (float *)KPR_SHMEM_AT(0U);
     uint32_t *col_ind_tile = (uint32_t *) KPR_SHMEM_AT(512U);
     uint32_t ri = gA.row_off[m_idx];
@@ -2383,8 +2433,8 @@ Klas_SPMM_g_spmm_f32_64x128x16(uint32_t rows,
     KPR_SHMEM_FITS(1024U);
     MUST(cudaFuncSetAttribute
          (__hoisted_24, cudaFuncAttributeMaxDynamicSharedMemorySize, 1024U));
-    KPR_KCALL(__hoisted_24, rows * ((cols + 63U) / 64U), 16U, 1024U, cols, gA,
-              row_indices, gB, gC);
+    KPR_KCALL(__hoisted_24, rows * (cols / 64U + (cols % 64U != 0U ? 1U : 0U)),
+              16U, 1024U, cols, gA, row_indices, gB, gC);
     MUST(cudaDeviceSynchronize());
 }
 
@@ -2397,8 +2447,10 @@ __hoisted_25(uint32_t cols,
              Kuiper_Sparse_Matrix_smatrix__float gA,
              uint32_t *row_indices, float *gB, float *gC)
 {
-    uint32_t m_idx = row_indices[blockIdx.x / ((cols + 63U) / 64U)];
-    uint32_t n_idx = blockIdx.x % ((cols + 63U) / 64U) * 64U;
+    uint32_t m_idx =
+        row_indices[blockIdx.x / (cols / 64U + (cols % 64U != 0U ? 1U : 0U))];
+    uint32_t n_idx =
+        blockIdx.x % (cols / 64U + (cols % 64U != 0U ? 1U : 0U)) * 64U;
     float *elems_tile = (float *)KPR_SHMEM_AT(0U);
     uint32_t *col_ind_tile = (uint32_t *) KPR_SHMEM_AT(512U);
     uint32_t ri = gA.row_off[m_idx];
@@ -2479,8 +2531,8 @@ Klas_SPMM_g_spmm_f32_64x128x32(uint32_t rows,
     KPR_SHMEM_FITS(1024U);
     MUST(cudaFuncSetAttribute
          (__hoisted_25, cudaFuncAttributeMaxDynamicSharedMemorySize, 1024U));
-    KPR_KCALL(__hoisted_25, rows * ((cols + 63U) / 64U), 32U, 1024U, cols, gA,
-              row_indices, gB, gC);
+    KPR_KCALL(__hoisted_25, rows * (cols / 64U + (cols % 64U != 0U ? 1U : 0U)),
+              32U, 1024U, cols, gA, row_indices, gB, gC);
     MUST(cudaDeviceSynchronize());
 }
 
@@ -2493,8 +2545,10 @@ __hoisted_26(uint32_t cols,
              Kuiper_Sparse_Matrix_smatrix__float gA,
              uint32_t *row_indices, float *gB, float *gC)
 {
-    uint32_t m_idx = row_indices[blockIdx.x / ((cols + 63U) / 64U)];
-    uint32_t n_idx = blockIdx.x % ((cols + 63U) / 64U) * 64U;
+    uint32_t m_idx =
+        row_indices[blockIdx.x / (cols / 64U + (cols % 64U != 0U ? 1U : 0U))];
+    uint32_t n_idx =
+        blockIdx.x % (cols / 64U + (cols % 64U != 0U ? 1U : 0U)) * 64U;
     float *elems_tile = (float *)KPR_SHMEM_AT(0U);
     uint32_t *col_ind_tile = (uint32_t *) KPR_SHMEM_AT(512U);
     uint32_t ri = gA.row_off[m_idx];
@@ -2574,8 +2628,8 @@ Klas_SPMM_g_spmm_f32_64x128x64(uint32_t rows,
     KPR_SHMEM_FITS(1024U);
     MUST(cudaFuncSetAttribute
          (__hoisted_26, cudaFuncAttributeMaxDynamicSharedMemorySize, 1024U));
-    KPR_KCALL(__hoisted_26, rows * ((cols + 63U) / 64U), 64U, 1024U, cols, gA,
-              row_indices, gB, gC);
+    KPR_KCALL(__hoisted_26, rows * (cols / 64U + (cols % 64U != 0U ? 1U : 0U)),
+              64U, 1024U, cols, gA, row_indices, gB, gC);
     MUST(cudaDeviceSynchronize());
 }
 
@@ -2588,8 +2642,10 @@ __hoisted_27(uint32_t cols,
              Kuiper_Sparse_Matrix_smatrix__float gA,
              uint32_t *row_indices, float *gB, float *gC)
 {
-    uint32_t m_idx = row_indices[blockIdx.x / ((cols + 63U) / 64U)];
-    uint32_t n_idx = blockIdx.x % ((cols + 63U) / 64U) * 64U;
+    uint32_t m_idx =
+        row_indices[blockIdx.x / (cols / 64U + (cols % 64U != 0U ? 1U : 0U))];
+    uint32_t n_idx =
+        blockIdx.x % (cols / 64U + (cols % 64U != 0U ? 1U : 0U)) * 64U;
     float *elems_tile = (float *)KPR_SHMEM_AT(0U);
     uint32_t *col_ind_tile = (uint32_t *) KPR_SHMEM_AT(1024U);
     uint32_t ri = gA.row_off[m_idx];
@@ -2670,8 +2726,8 @@ Klas_SPMM_g_spmm_f32_64x256x16(uint32_t rows,
     KPR_SHMEM_FITS(2048U);
     MUST(cudaFuncSetAttribute
          (__hoisted_27, cudaFuncAttributeMaxDynamicSharedMemorySize, 2048U));
-    KPR_KCALL(__hoisted_27, rows * ((cols + 63U) / 64U), 16U, 2048U, cols, gA,
-              row_indices, gB, gC);
+    KPR_KCALL(__hoisted_27, rows * (cols / 64U + (cols % 64U != 0U ? 1U : 0U)),
+              16U, 2048U, cols, gA, row_indices, gB, gC);
     MUST(cudaDeviceSynchronize());
 }
 
@@ -2684,8 +2740,10 @@ __hoisted_28(uint32_t cols,
              Kuiper_Sparse_Matrix_smatrix__float gA,
              uint32_t *row_indices, float *gB, float *gC)
 {
-    uint32_t m_idx = row_indices[blockIdx.x / ((cols + 63U) / 64U)];
-    uint32_t n_idx = blockIdx.x % ((cols + 63U) / 64U) * 64U;
+    uint32_t m_idx =
+        row_indices[blockIdx.x / (cols / 64U + (cols % 64U != 0U ? 1U : 0U))];
+    uint32_t n_idx =
+        blockIdx.x % (cols / 64U + (cols % 64U != 0U ? 1U : 0U)) * 64U;
     float *elems_tile = (float *)KPR_SHMEM_AT(0U);
     uint32_t *col_ind_tile = (uint32_t *) KPR_SHMEM_AT(1024U);
     uint32_t ri = gA.row_off[m_idx];
@@ -2766,8 +2824,8 @@ Klas_SPMM_g_spmm_f32_64x256x32(uint32_t rows,
     KPR_SHMEM_FITS(2048U);
     MUST(cudaFuncSetAttribute
          (__hoisted_28, cudaFuncAttributeMaxDynamicSharedMemorySize, 2048U));
-    KPR_KCALL(__hoisted_28, rows * ((cols + 63U) / 64U), 32U, 2048U, cols, gA,
-              row_indices, gB, gC);
+    KPR_KCALL(__hoisted_28, rows * (cols / 64U + (cols % 64U != 0U ? 1U : 0U)),
+              32U, 2048U, cols, gA, row_indices, gB, gC);
     MUST(cudaDeviceSynchronize());
 }
 
@@ -2780,8 +2838,10 @@ __hoisted_29(uint32_t cols,
              Kuiper_Sparse_Matrix_smatrix__float gA,
              uint32_t *row_indices, float *gB, float *gC)
 {
-    uint32_t m_idx = row_indices[blockIdx.x / ((cols + 63U) / 64U)];
-    uint32_t n_idx = blockIdx.x % ((cols + 63U) / 64U) * 64U;
+    uint32_t m_idx =
+        row_indices[blockIdx.x / (cols / 64U + (cols % 64U != 0U ? 1U : 0U))];
+    uint32_t n_idx =
+        blockIdx.x % (cols / 64U + (cols % 64U != 0U ? 1U : 0U)) * 64U;
     float *elems_tile = (float *)KPR_SHMEM_AT(0U);
     uint32_t *col_ind_tile = (uint32_t *) KPR_SHMEM_AT(1024U);
     uint32_t ri = gA.row_off[m_idx];
@@ -2861,8 +2921,8 @@ Klas_SPMM_g_spmm_f32_64x256x64(uint32_t rows,
     KPR_SHMEM_FITS(2048U);
     MUST(cudaFuncSetAttribute
          (__hoisted_29, cudaFuncAttributeMaxDynamicSharedMemorySize, 2048U));
-    KPR_KCALL(__hoisted_29, rows * ((cols + 63U) / 64U), 64U, 2048U, cols, gA,
-              row_indices, gB, gC);
+    KPR_KCALL(__hoisted_29, rows * (cols / 64U + (cols % 64U != 0U ? 1U : 0U)),
+              64U, 2048U, cols, gA, row_indices, gB, gC);
     MUST(cudaDeviceSynchronize());
 }
 
@@ -2875,8 +2935,10 @@ __hoisted_30(uint32_t cols,
              Kuiper_Sparse_Matrix_smatrix__float gA,
              uint32_t *row_indices, float *gB, float *gC)
 {
-    uint32_t m_idx = row_indices[blockIdx.x / ((cols + 63U) / 64U)];
-    uint32_t n_idx = blockIdx.x % ((cols + 63U) / 64U) * 64U;
+    uint32_t m_idx =
+        row_indices[blockIdx.x / (cols / 64U + (cols % 64U != 0U ? 1U : 0U))];
+    uint32_t n_idx =
+        blockIdx.x % (cols / 64U + (cols % 64U != 0U ? 1U : 0U)) * 64U;
     float *elems_tile = (float *)KPR_SHMEM_AT(0U);
     uint32_t *col_ind_tile = (uint32_t *) KPR_SHMEM_AT(2048U);
     uint32_t ri = gA.row_off[m_idx];
@@ -2957,8 +3019,8 @@ Klas_SPMM_g_spmm_f32_64x512x16(uint32_t rows,
     KPR_SHMEM_FITS(4096U);
     MUST(cudaFuncSetAttribute
          (__hoisted_30, cudaFuncAttributeMaxDynamicSharedMemorySize, 4096U));
-    KPR_KCALL(__hoisted_30, rows * ((cols + 63U) / 64U), 16U, 4096U, cols, gA,
-              row_indices, gB, gC);
+    KPR_KCALL(__hoisted_30, rows * (cols / 64U + (cols % 64U != 0U ? 1U : 0U)),
+              16U, 4096U, cols, gA, row_indices, gB, gC);
     MUST(cudaDeviceSynchronize());
 }
 
@@ -2971,8 +3033,10 @@ __hoisted_31(uint32_t cols,
              Kuiper_Sparse_Matrix_smatrix__float gA,
              uint32_t *row_indices, float *gB, float *gC)
 {
-    uint32_t m_idx = row_indices[blockIdx.x / ((cols + 63U) / 64U)];
-    uint32_t n_idx = blockIdx.x % ((cols + 63U) / 64U) * 64U;
+    uint32_t m_idx =
+        row_indices[blockIdx.x / (cols / 64U + (cols % 64U != 0U ? 1U : 0U))];
+    uint32_t n_idx =
+        blockIdx.x % (cols / 64U + (cols % 64U != 0U ? 1U : 0U)) * 64U;
     float *elems_tile = (float *)KPR_SHMEM_AT(0U);
     uint32_t *col_ind_tile = (uint32_t *) KPR_SHMEM_AT(2048U);
     uint32_t ri = gA.row_off[m_idx];
@@ -3053,8 +3117,8 @@ Klas_SPMM_g_spmm_f32_64x512x32(uint32_t rows,
     KPR_SHMEM_FITS(4096U);
     MUST(cudaFuncSetAttribute
          (__hoisted_31, cudaFuncAttributeMaxDynamicSharedMemorySize, 4096U));
-    KPR_KCALL(__hoisted_31, rows * ((cols + 63U) / 64U), 32U, 4096U, cols, gA,
-              row_indices, gB, gC);
+    KPR_KCALL(__hoisted_31, rows * (cols / 64U + (cols % 64U != 0U ? 1U : 0U)),
+              32U, 4096U, cols, gA, row_indices, gB, gC);
     MUST(cudaDeviceSynchronize());
 }
 
@@ -3067,8 +3131,10 @@ __hoisted_32(uint32_t cols,
              Kuiper_Sparse_Matrix_smatrix__float gA,
              uint32_t *row_indices, float *gB, float *gC)
 {
-    uint32_t m_idx = row_indices[blockIdx.x / ((cols + 63U) / 64U)];
-    uint32_t n_idx = blockIdx.x % ((cols + 63U) / 64U) * 64U;
+    uint32_t m_idx =
+        row_indices[blockIdx.x / (cols / 64U + (cols % 64U != 0U ? 1U : 0U))];
+    uint32_t n_idx =
+        blockIdx.x % (cols / 64U + (cols % 64U != 0U ? 1U : 0U)) * 64U;
     float *elems_tile = (float *)KPR_SHMEM_AT(0U);
     uint32_t *col_ind_tile = (uint32_t *) KPR_SHMEM_AT(2048U);
     uint32_t ri = gA.row_off[m_idx];
@@ -3148,8 +3214,8 @@ Klas_SPMM_g_spmm_f32_64x512x64(uint32_t rows,
     KPR_SHMEM_FITS(4096U);
     MUST(cudaFuncSetAttribute
          (__hoisted_32, cudaFuncAttributeMaxDynamicSharedMemorySize, 4096U));
-    KPR_KCALL(__hoisted_32, rows * ((cols + 63U) / 64U), 64U, 4096U, cols, gA,
-              row_indices, gB, gC);
+    KPR_KCALL(__hoisted_32, rows * (cols / 64U + (cols % 64U != 0U ? 1U : 0U)),
+              64U, 4096U, cols, gA, row_indices, gB, gC);
     MUST(cudaDeviceSynchronize());
 }
 
@@ -3162,8 +3228,10 @@ __hoisted_33(uint32_t cols,
              Kuiper_Sparse_Matrix_smatrix__float gA,
              uint32_t *row_indices, float *gB, float *gC)
 {
-    uint32_t m_idx = row_indices[blockIdx.x / ((cols + 127U) / 128U)];
-    uint32_t n_idx = blockIdx.x % ((cols + 127U) / 128U) * 128U;
+    uint32_t m_idx =
+        row_indices[blockIdx.x / (cols / 128U + (cols % 128U != 0U ? 1U : 0U))];
+    uint32_t n_idx =
+        blockIdx.x % (cols / 128U + (cols % 128U != 0U ? 1U : 0U)) * 128U;
     float *elems_tile = (float *)KPR_SHMEM_AT(0U);
     uint32_t *col_ind_tile = (uint32_t *) KPR_SHMEM_AT(64U);
     uint32_t ri = gA.row_off[m_idx];
@@ -3244,8 +3312,9 @@ Klas_SPMM_g_spmm_f32_128x16x16(uint32_t rows,
     KPR_SHMEM_FITS(128U);
     MUST(cudaFuncSetAttribute
          (__hoisted_33, cudaFuncAttributeMaxDynamicSharedMemorySize, 128U));
-    KPR_KCALL(__hoisted_33, rows * ((cols + 127U) / 128U), 16U, 128U, cols, gA,
-              row_indices, gB, gC);
+    KPR_KCALL(__hoisted_33,
+              rows * (cols / 128U + (cols % 128U != 0U ? 1U : 0U)), 16U, 128U,
+              cols, gA, row_indices, gB, gC);
     MUST(cudaDeviceSynchronize());
 }
 
@@ -3258,8 +3327,10 @@ __hoisted_34(uint32_t cols,
              Kuiper_Sparse_Matrix_smatrix__float gA,
              uint32_t *row_indices, float *gB, float *gC)
 {
-    uint32_t m_idx = row_indices[blockIdx.x / ((cols + 127U) / 128U)];
-    uint32_t n_idx = blockIdx.x % ((cols + 127U) / 128U) * 128U;
+    uint32_t m_idx =
+        row_indices[blockIdx.x / (cols / 128U + (cols % 128U != 0U ? 1U : 0U))];
+    uint32_t n_idx =
+        blockIdx.x % (cols / 128U + (cols % 128U != 0U ? 1U : 0U)) * 128U;
     float *elems_tile = (float *)KPR_SHMEM_AT(0U);
     uint32_t *col_ind_tile = (uint32_t *) KPR_SHMEM_AT(128U);
     uint32_t ri = gA.row_off[m_idx];
@@ -3340,8 +3411,9 @@ Klas_SPMM_g_spmm_f32_128x32x16(uint32_t rows,
     KPR_SHMEM_FITS(256U);
     MUST(cudaFuncSetAttribute
          (__hoisted_34, cudaFuncAttributeMaxDynamicSharedMemorySize, 256U));
-    KPR_KCALL(__hoisted_34, rows * ((cols + 127U) / 128U), 16U, 256U, cols, gA,
-              row_indices, gB, gC);
+    KPR_KCALL(__hoisted_34,
+              rows * (cols / 128U + (cols % 128U != 0U ? 1U : 0U)), 16U, 256U,
+              cols, gA, row_indices, gB, gC);
     MUST(cudaDeviceSynchronize());
 }
 
@@ -3354,8 +3426,10 @@ __hoisted_35(uint32_t cols,
              Kuiper_Sparse_Matrix_smatrix__float gA,
              uint32_t *row_indices, float *gB, float *gC)
 {
-    uint32_t m_idx = row_indices[blockIdx.x / ((cols + 127U) / 128U)];
-    uint32_t n_idx = blockIdx.x % ((cols + 127U) / 128U) * 128U;
+    uint32_t m_idx =
+        row_indices[blockIdx.x / (cols / 128U + (cols % 128U != 0U ? 1U : 0U))];
+    uint32_t n_idx =
+        blockIdx.x % (cols / 128U + (cols % 128U != 0U ? 1U : 0U)) * 128U;
     float *elems_tile = (float *)KPR_SHMEM_AT(0U);
     uint32_t *col_ind_tile = (uint32_t *) KPR_SHMEM_AT(128U);
     uint32_t ri = gA.row_off[m_idx];
@@ -3436,8 +3510,9 @@ Klas_SPMM_g_spmm_f32_128x32x32(uint32_t rows,
     KPR_SHMEM_FITS(256U);
     MUST(cudaFuncSetAttribute
          (__hoisted_35, cudaFuncAttributeMaxDynamicSharedMemorySize, 256U));
-    KPR_KCALL(__hoisted_35, rows * ((cols + 127U) / 128U), 32U, 256U, cols, gA,
-              row_indices, gB, gC);
+    KPR_KCALL(__hoisted_35,
+              rows * (cols / 128U + (cols % 128U != 0U ? 1U : 0U)), 32U, 256U,
+              cols, gA, row_indices, gB, gC);
     MUST(cudaDeviceSynchronize());
 }
 
@@ -3450,8 +3525,10 @@ __hoisted_36(uint32_t cols,
              Kuiper_Sparse_Matrix_smatrix__float gA,
              uint32_t *row_indices, float *gB, float *gC)
 {
-    uint32_t m_idx = row_indices[blockIdx.x / ((cols + 127U) / 128U)];
-    uint32_t n_idx = blockIdx.x % ((cols + 127U) / 128U) * 128U;
+    uint32_t m_idx =
+        row_indices[blockIdx.x / (cols / 128U + (cols % 128U != 0U ? 1U : 0U))];
+    uint32_t n_idx =
+        blockIdx.x % (cols / 128U + (cols % 128U != 0U ? 1U : 0U)) * 128U;
     float *elems_tile = (float *)KPR_SHMEM_AT(0U);
     uint32_t *col_ind_tile = (uint32_t *) KPR_SHMEM_AT(256U);
     uint32_t ri = gA.row_off[m_idx];
@@ -3532,8 +3609,9 @@ Klas_SPMM_g_spmm_f32_128x64x16(uint32_t rows,
     KPR_SHMEM_FITS(512U);
     MUST(cudaFuncSetAttribute
          (__hoisted_36, cudaFuncAttributeMaxDynamicSharedMemorySize, 512U));
-    KPR_KCALL(__hoisted_36, rows * ((cols + 127U) / 128U), 16U, 512U, cols, gA,
-              row_indices, gB, gC);
+    KPR_KCALL(__hoisted_36,
+              rows * (cols / 128U + (cols % 128U != 0U ? 1U : 0U)), 16U, 512U,
+              cols, gA, row_indices, gB, gC);
     MUST(cudaDeviceSynchronize());
 }
 
@@ -3546,8 +3624,10 @@ __hoisted_37(uint32_t cols,
              Kuiper_Sparse_Matrix_smatrix__float gA,
              uint32_t *row_indices, float *gB, float *gC)
 {
-    uint32_t m_idx = row_indices[blockIdx.x / ((cols + 127U) / 128U)];
-    uint32_t n_idx = blockIdx.x % ((cols + 127U) / 128U) * 128U;
+    uint32_t m_idx =
+        row_indices[blockIdx.x / (cols / 128U + (cols % 128U != 0U ? 1U : 0U))];
+    uint32_t n_idx =
+        blockIdx.x % (cols / 128U + (cols % 128U != 0U ? 1U : 0U)) * 128U;
     float *elems_tile = (float *)KPR_SHMEM_AT(0U);
     uint32_t *col_ind_tile = (uint32_t *) KPR_SHMEM_AT(256U);
     uint32_t ri = gA.row_off[m_idx];
@@ -3628,8 +3708,9 @@ Klas_SPMM_g_spmm_f32_128x64x32(uint32_t rows,
     KPR_SHMEM_FITS(512U);
     MUST(cudaFuncSetAttribute
          (__hoisted_37, cudaFuncAttributeMaxDynamicSharedMemorySize, 512U));
-    KPR_KCALL(__hoisted_37, rows * ((cols + 127U) / 128U), 32U, 512U, cols, gA,
-              row_indices, gB, gC);
+    KPR_KCALL(__hoisted_37,
+              rows * (cols / 128U + (cols % 128U != 0U ? 1U : 0U)), 32U, 512U,
+              cols, gA, row_indices, gB, gC);
     MUST(cudaDeviceSynchronize());
 }
 
@@ -3642,8 +3723,10 @@ __hoisted_38(uint32_t cols,
              Kuiper_Sparse_Matrix_smatrix__float gA,
              uint32_t *row_indices, float *gB, float *gC)
 {
-    uint32_t m_idx = row_indices[blockIdx.x / ((cols + 127U) / 128U)];
-    uint32_t n_idx = blockIdx.x % ((cols + 127U) / 128U) * 128U;
+    uint32_t m_idx =
+        row_indices[blockIdx.x / (cols / 128U + (cols % 128U != 0U ? 1U : 0U))];
+    uint32_t n_idx =
+        blockIdx.x % (cols / 128U + (cols % 128U != 0U ? 1U : 0U)) * 128U;
     float *elems_tile = (float *)KPR_SHMEM_AT(0U);
     uint32_t *col_ind_tile = (uint32_t *) KPR_SHMEM_AT(256U);
     uint32_t ri = gA.row_off[m_idx];
@@ -3724,8 +3807,9 @@ Klas_SPMM_g_spmm_f32_128x64x64(uint32_t rows,
     KPR_SHMEM_FITS(512U);
     MUST(cudaFuncSetAttribute
          (__hoisted_38, cudaFuncAttributeMaxDynamicSharedMemorySize, 512U));
-    KPR_KCALL(__hoisted_38, rows * ((cols + 127U) / 128U), 64U, 512U, cols, gA,
-              row_indices, gB, gC);
+    KPR_KCALL(__hoisted_38,
+              rows * (cols / 128U + (cols % 128U != 0U ? 1U : 0U)), 64U, 512U,
+              cols, gA, row_indices, gB, gC);
     MUST(cudaDeviceSynchronize());
 }
 
@@ -3738,8 +3822,10 @@ __hoisted_39(uint32_t cols,
              Kuiper_Sparse_Matrix_smatrix__float gA,
              uint32_t *row_indices, float *gB, float *gC)
 {
-    uint32_t m_idx = row_indices[blockIdx.x / ((cols + 127U) / 128U)];
-    uint32_t n_idx = blockIdx.x % ((cols + 127U) / 128U) * 128U;
+    uint32_t m_idx =
+        row_indices[blockIdx.x / (cols / 128U + (cols % 128U != 0U ? 1U : 0U))];
+    uint32_t n_idx =
+        blockIdx.x % (cols / 128U + (cols % 128U != 0U ? 1U : 0U)) * 128U;
     float *elems_tile = (float *)KPR_SHMEM_AT(0U);
     uint32_t *col_ind_tile = (uint32_t *) KPR_SHMEM_AT(512U);
     uint32_t ri = gA.row_off[m_idx];
@@ -3820,8 +3906,9 @@ Klas_SPMM_g_spmm_f32_128x128x16(uint32_t rows,
     KPR_SHMEM_FITS(1024U);
     MUST(cudaFuncSetAttribute
          (__hoisted_39, cudaFuncAttributeMaxDynamicSharedMemorySize, 1024U));
-    KPR_KCALL(__hoisted_39, rows * ((cols + 127U) / 128U), 16U, 1024U, cols, gA,
-              row_indices, gB, gC);
+    KPR_KCALL(__hoisted_39,
+              rows * (cols / 128U + (cols % 128U != 0U ? 1U : 0U)), 16U, 1024U,
+              cols, gA, row_indices, gB, gC);
     MUST(cudaDeviceSynchronize());
 }
 
@@ -3834,8 +3921,10 @@ __hoisted_40(uint32_t cols,
              Kuiper_Sparse_Matrix_smatrix__float gA,
              uint32_t *row_indices, float *gB, float *gC)
 {
-    uint32_t m_idx = row_indices[blockIdx.x / ((cols + 127U) / 128U)];
-    uint32_t n_idx = blockIdx.x % ((cols + 127U) / 128U) * 128U;
+    uint32_t m_idx =
+        row_indices[blockIdx.x / (cols / 128U + (cols % 128U != 0U ? 1U : 0U))];
+    uint32_t n_idx =
+        blockIdx.x % (cols / 128U + (cols % 128U != 0U ? 1U : 0U)) * 128U;
     float *elems_tile = (float *)KPR_SHMEM_AT(0U);
     uint32_t *col_ind_tile = (uint32_t *) KPR_SHMEM_AT(512U);
     uint32_t ri = gA.row_off[m_idx];
@@ -3916,8 +4005,9 @@ Klas_SPMM_g_spmm_f32_128x128x32(uint32_t rows,
     KPR_SHMEM_FITS(1024U);
     MUST(cudaFuncSetAttribute
          (__hoisted_40, cudaFuncAttributeMaxDynamicSharedMemorySize, 1024U));
-    KPR_KCALL(__hoisted_40, rows * ((cols + 127U) / 128U), 32U, 1024U, cols, gA,
-              row_indices, gB, gC);
+    KPR_KCALL(__hoisted_40,
+              rows * (cols / 128U + (cols % 128U != 0U ? 1U : 0U)), 32U, 1024U,
+              cols, gA, row_indices, gB, gC);
     MUST(cudaDeviceSynchronize());
 }
 
@@ -3930,8 +4020,10 @@ __hoisted_41(uint32_t cols,
              Kuiper_Sparse_Matrix_smatrix__float gA,
              uint32_t *row_indices, float *gB, float *gC)
 {
-    uint32_t m_idx = row_indices[blockIdx.x / ((cols + 127U) / 128U)];
-    uint32_t n_idx = blockIdx.x % ((cols + 127U) / 128U) * 128U;
+    uint32_t m_idx =
+        row_indices[blockIdx.x / (cols / 128U + (cols % 128U != 0U ? 1U : 0U))];
+    uint32_t n_idx =
+        blockIdx.x % (cols / 128U + (cols % 128U != 0U ? 1U : 0U)) * 128U;
     float *elems_tile = (float *)KPR_SHMEM_AT(0U);
     uint32_t *col_ind_tile = (uint32_t *) KPR_SHMEM_AT(512U);
     uint32_t ri = gA.row_off[m_idx];
@@ -4012,8 +4104,9 @@ Klas_SPMM_g_spmm_f32_128x128x64(uint32_t rows,
     KPR_SHMEM_FITS(1024U);
     MUST(cudaFuncSetAttribute
          (__hoisted_41, cudaFuncAttributeMaxDynamicSharedMemorySize, 1024U));
-    KPR_KCALL(__hoisted_41, rows * ((cols + 127U) / 128U), 64U, 1024U, cols, gA,
-              row_indices, gB, gC);
+    KPR_KCALL(__hoisted_41,
+              rows * (cols / 128U + (cols % 128U != 0U ? 1U : 0U)), 64U, 1024U,
+              cols, gA, row_indices, gB, gC);
     MUST(cudaDeviceSynchronize());
 }
 
@@ -4026,8 +4119,10 @@ __hoisted_42(uint32_t cols,
              Kuiper_Sparse_Matrix_smatrix__float gA,
              uint32_t *row_indices, float *gB, float *gC)
 {
-    uint32_t m_idx = row_indices[blockIdx.x / ((cols + 127U) / 128U)];
-    uint32_t n_idx = blockIdx.x % ((cols + 127U) / 128U) * 128U;
+    uint32_t m_idx =
+        row_indices[blockIdx.x / (cols / 128U + (cols % 128U != 0U ? 1U : 0U))];
+    uint32_t n_idx =
+        blockIdx.x % (cols / 128U + (cols % 128U != 0U ? 1U : 0U)) * 128U;
     float *elems_tile = (float *)KPR_SHMEM_AT(0U);
     uint32_t *col_ind_tile = (uint32_t *) KPR_SHMEM_AT(512U);
     uint32_t ri = gA.row_off[m_idx];
@@ -4107,8 +4202,9 @@ Klas_SPMM_g_spmm_f32_128x128x128(uint32_t rows,
     KPR_SHMEM_FITS(1024U);
     MUST(cudaFuncSetAttribute
          (__hoisted_42, cudaFuncAttributeMaxDynamicSharedMemorySize, 1024U));
-    KPR_KCALL(__hoisted_42, rows * ((cols + 127U) / 128U), 128U, 1024U, cols,
-              gA, row_indices, gB, gC);
+    KPR_KCALL(__hoisted_42,
+              rows * (cols / 128U + (cols % 128U != 0U ? 1U : 0U)), 128U, 1024U,
+              cols, gA, row_indices, gB, gC);
     MUST(cudaDeviceSynchronize());
 }
 
@@ -4121,8 +4217,10 @@ __hoisted_43(uint32_t cols,
              Kuiper_Sparse_Matrix_smatrix__float gA,
              uint32_t *row_indices, float *gB, float *gC)
 {
-    uint32_t m_idx = row_indices[blockIdx.x / ((cols + 127U) / 128U)];
-    uint32_t n_idx = blockIdx.x % ((cols + 127U) / 128U) * 128U;
+    uint32_t m_idx =
+        row_indices[blockIdx.x / (cols / 128U + (cols % 128U != 0U ? 1U : 0U))];
+    uint32_t n_idx =
+        blockIdx.x % (cols / 128U + (cols % 128U != 0U ? 1U : 0U)) * 128U;
     float *elems_tile = (float *)KPR_SHMEM_AT(0U);
     uint32_t *col_ind_tile = (uint32_t *) KPR_SHMEM_AT(1024U);
     uint32_t ri = gA.row_off[m_idx];
@@ -4203,8 +4301,9 @@ Klas_SPMM_g_spmm_f32_128x256x16(uint32_t rows,
     KPR_SHMEM_FITS(2048U);
     MUST(cudaFuncSetAttribute
          (__hoisted_43, cudaFuncAttributeMaxDynamicSharedMemorySize, 2048U));
-    KPR_KCALL(__hoisted_43, rows * ((cols + 127U) / 128U), 16U, 2048U, cols, gA,
-              row_indices, gB, gC);
+    KPR_KCALL(__hoisted_43,
+              rows * (cols / 128U + (cols % 128U != 0U ? 1U : 0U)), 16U, 2048U,
+              cols, gA, row_indices, gB, gC);
     MUST(cudaDeviceSynchronize());
 }
 
@@ -4217,8 +4316,10 @@ __hoisted_44(uint32_t cols,
              Kuiper_Sparse_Matrix_smatrix__float gA,
              uint32_t *row_indices, float *gB, float *gC)
 {
-    uint32_t m_idx = row_indices[blockIdx.x / ((cols + 127U) / 128U)];
-    uint32_t n_idx = blockIdx.x % ((cols + 127U) / 128U) * 128U;
+    uint32_t m_idx =
+        row_indices[blockIdx.x / (cols / 128U + (cols % 128U != 0U ? 1U : 0U))];
+    uint32_t n_idx =
+        blockIdx.x % (cols / 128U + (cols % 128U != 0U ? 1U : 0U)) * 128U;
     float *elems_tile = (float *)KPR_SHMEM_AT(0U);
     uint32_t *col_ind_tile = (uint32_t *) KPR_SHMEM_AT(1024U);
     uint32_t ri = gA.row_off[m_idx];
@@ -4299,8 +4400,9 @@ Klas_SPMM_g_spmm_f32_128x256x32(uint32_t rows,
     KPR_SHMEM_FITS(2048U);
     MUST(cudaFuncSetAttribute
          (__hoisted_44, cudaFuncAttributeMaxDynamicSharedMemorySize, 2048U));
-    KPR_KCALL(__hoisted_44, rows * ((cols + 127U) / 128U), 32U, 2048U, cols, gA,
-              row_indices, gB, gC);
+    KPR_KCALL(__hoisted_44,
+              rows * (cols / 128U + (cols % 128U != 0U ? 1U : 0U)), 32U, 2048U,
+              cols, gA, row_indices, gB, gC);
     MUST(cudaDeviceSynchronize());
 }
 
@@ -4313,8 +4415,10 @@ __hoisted_45(uint32_t cols,
              Kuiper_Sparse_Matrix_smatrix__float gA,
              uint32_t *row_indices, float *gB, float *gC)
 {
-    uint32_t m_idx = row_indices[blockIdx.x / ((cols + 127U) / 128U)];
-    uint32_t n_idx = blockIdx.x % ((cols + 127U) / 128U) * 128U;
+    uint32_t m_idx =
+        row_indices[blockIdx.x / (cols / 128U + (cols % 128U != 0U ? 1U : 0U))];
+    uint32_t n_idx =
+        blockIdx.x % (cols / 128U + (cols % 128U != 0U ? 1U : 0U)) * 128U;
     float *elems_tile = (float *)KPR_SHMEM_AT(0U);
     uint32_t *col_ind_tile = (uint32_t *) KPR_SHMEM_AT(1024U);
     uint32_t ri = gA.row_off[m_idx];
@@ -4395,8 +4499,9 @@ Klas_SPMM_g_spmm_f32_128x256x64(uint32_t rows,
     KPR_SHMEM_FITS(2048U);
     MUST(cudaFuncSetAttribute
          (__hoisted_45, cudaFuncAttributeMaxDynamicSharedMemorySize, 2048U));
-    KPR_KCALL(__hoisted_45, rows * ((cols + 127U) / 128U), 64U, 2048U, cols, gA,
-              row_indices, gB, gC);
+    KPR_KCALL(__hoisted_45,
+              rows * (cols / 128U + (cols % 128U != 0U ? 1U : 0U)), 64U, 2048U,
+              cols, gA, row_indices, gB, gC);
     MUST(cudaDeviceSynchronize());
 }
 
@@ -4409,8 +4514,10 @@ __hoisted_46(uint32_t cols,
              Kuiper_Sparse_Matrix_smatrix__float gA,
              uint32_t *row_indices, float *gB, float *gC)
 {
-    uint32_t m_idx = row_indices[blockIdx.x / ((cols + 127U) / 128U)];
-    uint32_t n_idx = blockIdx.x % ((cols + 127U) / 128U) * 128U;
+    uint32_t m_idx =
+        row_indices[blockIdx.x / (cols / 128U + (cols % 128U != 0U ? 1U : 0U))];
+    uint32_t n_idx =
+        blockIdx.x % (cols / 128U + (cols % 128U != 0U ? 1U : 0U)) * 128U;
     float *elems_tile = (float *)KPR_SHMEM_AT(0U);
     uint32_t *col_ind_tile = (uint32_t *) KPR_SHMEM_AT(1024U);
     uint32_t ri = gA.row_off[m_idx];
@@ -4490,8 +4597,9 @@ Klas_SPMM_g_spmm_f32_128x256x128(uint32_t rows,
     KPR_SHMEM_FITS(2048U);
     MUST(cudaFuncSetAttribute
          (__hoisted_46, cudaFuncAttributeMaxDynamicSharedMemorySize, 2048U));
-    KPR_KCALL(__hoisted_46, rows * ((cols + 127U) / 128U), 128U, 2048U, cols,
-              gA, row_indices, gB, gC);
+    KPR_KCALL(__hoisted_46,
+              rows * (cols / 128U + (cols % 128U != 0U ? 1U : 0U)), 128U, 2048U,
+              cols, gA, row_indices, gB, gC);
     MUST(cudaDeviceSynchronize());
 }
 
@@ -4504,8 +4612,10 @@ __hoisted_47(uint32_t cols,
              Kuiper_Sparse_Matrix_smatrix__float gA,
              uint32_t *row_indices, float *gB, float *gC)
 {
-    uint32_t m_idx = row_indices[blockIdx.x / ((cols + 127U) / 128U)];
-    uint32_t n_idx = blockIdx.x % ((cols + 127U) / 128U) * 128U;
+    uint32_t m_idx =
+        row_indices[blockIdx.x / (cols / 128U + (cols % 128U != 0U ? 1U : 0U))];
+    uint32_t n_idx =
+        blockIdx.x % (cols / 128U + (cols % 128U != 0U ? 1U : 0U)) * 128U;
     float *elems_tile = (float *)KPR_SHMEM_AT(0U);
     uint32_t *col_ind_tile = (uint32_t *) KPR_SHMEM_AT(2048U);
     uint32_t ri = gA.row_off[m_idx];
@@ -4586,8 +4696,9 @@ Klas_SPMM_g_spmm_f32_128x512x16(uint32_t rows,
     KPR_SHMEM_FITS(4096U);
     MUST(cudaFuncSetAttribute
          (__hoisted_47, cudaFuncAttributeMaxDynamicSharedMemorySize, 4096U));
-    KPR_KCALL(__hoisted_47, rows * ((cols + 127U) / 128U), 16U, 4096U, cols, gA,
-              row_indices, gB, gC);
+    KPR_KCALL(__hoisted_47,
+              rows * (cols / 128U + (cols % 128U != 0U ? 1U : 0U)), 16U, 4096U,
+              cols, gA, row_indices, gB, gC);
     MUST(cudaDeviceSynchronize());
 }
 
@@ -4600,8 +4711,10 @@ __hoisted_48(uint32_t cols,
              Kuiper_Sparse_Matrix_smatrix__float gA,
              uint32_t *row_indices, float *gB, float *gC)
 {
-    uint32_t m_idx = row_indices[blockIdx.x / ((cols + 127U) / 128U)];
-    uint32_t n_idx = blockIdx.x % ((cols + 127U) / 128U) * 128U;
+    uint32_t m_idx =
+        row_indices[blockIdx.x / (cols / 128U + (cols % 128U != 0U ? 1U : 0U))];
+    uint32_t n_idx =
+        blockIdx.x % (cols / 128U + (cols % 128U != 0U ? 1U : 0U)) * 128U;
     float *elems_tile = (float *)KPR_SHMEM_AT(0U);
     uint32_t *col_ind_tile = (uint32_t *) KPR_SHMEM_AT(2048U);
     uint32_t ri = gA.row_off[m_idx];
@@ -4682,8 +4795,9 @@ Klas_SPMM_g_spmm_f32_128x512x32(uint32_t rows,
     KPR_SHMEM_FITS(4096U);
     MUST(cudaFuncSetAttribute
          (__hoisted_48, cudaFuncAttributeMaxDynamicSharedMemorySize, 4096U));
-    KPR_KCALL(__hoisted_48, rows * ((cols + 127U) / 128U), 32U, 4096U, cols, gA,
-              row_indices, gB, gC);
+    KPR_KCALL(__hoisted_48,
+              rows * (cols / 128U + (cols % 128U != 0U ? 1U : 0U)), 32U, 4096U,
+              cols, gA, row_indices, gB, gC);
     MUST(cudaDeviceSynchronize());
 }
 
@@ -4696,8 +4810,10 @@ __hoisted_49(uint32_t cols,
              Kuiper_Sparse_Matrix_smatrix__float gA,
              uint32_t *row_indices, float *gB, float *gC)
 {
-    uint32_t m_idx = row_indices[blockIdx.x / ((cols + 127U) / 128U)];
-    uint32_t n_idx = blockIdx.x % ((cols + 127U) / 128U) * 128U;
+    uint32_t m_idx =
+        row_indices[blockIdx.x / (cols / 128U + (cols % 128U != 0U ? 1U : 0U))];
+    uint32_t n_idx =
+        blockIdx.x % (cols / 128U + (cols % 128U != 0U ? 1U : 0U)) * 128U;
     float *elems_tile = (float *)KPR_SHMEM_AT(0U);
     uint32_t *col_ind_tile = (uint32_t *) KPR_SHMEM_AT(2048U);
     uint32_t ri = gA.row_off[m_idx];
@@ -4778,8 +4894,9 @@ Klas_SPMM_g_spmm_f32_128x512x64(uint32_t rows,
     KPR_SHMEM_FITS(4096U);
     MUST(cudaFuncSetAttribute
          (__hoisted_49, cudaFuncAttributeMaxDynamicSharedMemorySize, 4096U));
-    KPR_KCALL(__hoisted_49, rows * ((cols + 127U) / 128U), 64U, 4096U, cols, gA,
-              row_indices, gB, gC);
+    KPR_KCALL(__hoisted_49,
+              rows * (cols / 128U + (cols % 128U != 0U ? 1U : 0U)), 64U, 4096U,
+              cols, gA, row_indices, gB, gC);
     MUST(cudaDeviceSynchronize());
 }
 
@@ -4792,8 +4909,10 @@ __hoisted_50(uint32_t cols,
              Kuiper_Sparse_Matrix_smatrix__float gA,
              uint32_t *row_indices, float *gB, float *gC)
 {
-    uint32_t m_idx = row_indices[blockIdx.x / ((cols + 127U) / 128U)];
-    uint32_t n_idx = blockIdx.x % ((cols + 127U) / 128U) * 128U;
+    uint32_t m_idx =
+        row_indices[blockIdx.x / (cols / 128U + (cols % 128U != 0U ? 1U : 0U))];
+    uint32_t n_idx =
+        blockIdx.x % (cols / 128U + (cols % 128U != 0U ? 1U : 0U)) * 128U;
     float *elems_tile = (float *)KPR_SHMEM_AT(0U);
     uint32_t *col_ind_tile = (uint32_t *) KPR_SHMEM_AT(2048U);
     uint32_t ri = gA.row_off[m_idx];
@@ -4873,8 +4992,9 @@ Klas_SPMM_g_spmm_f32_128x512x128(uint32_t rows,
     KPR_SHMEM_FITS(4096U);
     MUST(cudaFuncSetAttribute
          (__hoisted_50, cudaFuncAttributeMaxDynamicSharedMemorySize, 4096U));
-    KPR_KCALL(__hoisted_50, rows * ((cols + 127U) / 128U), 128U, 4096U, cols,
-              gA, row_indices, gB, gC);
+    KPR_KCALL(__hoisted_50,
+              rows * (cols / 128U + (cols % 128U != 0U ? 1U : 0U)), 128U, 4096U,
+              cols, gA, row_indices, gB, gC);
     MUST(cudaDeviceSynchronize());
 }
 
@@ -4887,8 +5007,10 @@ __hoisted_51(uint32_t cols,
              Kuiper_Sparse_Matrix_smatrix__float gA,
              uint32_t *row_indices, float *gB, float *gC)
 {
-    uint32_t m_idx = row_indices[blockIdx.x / ((cols + 255U) / 256U)];
-    uint32_t n_idx = blockIdx.x % ((cols + 255U) / 256U) * 256U;
+    uint32_t m_idx =
+        row_indices[blockIdx.x / (cols / 256U + (cols % 256U != 0U ? 1U : 0U))];
+    uint32_t n_idx =
+        blockIdx.x % (cols / 256U + (cols % 256U != 0U ? 1U : 0U)) * 256U;
     float *elems_tile = (float *)KPR_SHMEM_AT(0U);
     uint32_t *col_ind_tile = (uint32_t *) KPR_SHMEM_AT(64U);
     uint32_t ri = gA.row_off[m_idx];
@@ -4969,8 +5091,9 @@ Klas_SPMM_g_spmm_f32_256x16x16(uint32_t rows,
     KPR_SHMEM_FITS(128U);
     MUST(cudaFuncSetAttribute
          (__hoisted_51, cudaFuncAttributeMaxDynamicSharedMemorySize, 128U));
-    KPR_KCALL(__hoisted_51, rows * ((cols + 255U) / 256U), 16U, 128U, cols, gA,
-              row_indices, gB, gC);
+    KPR_KCALL(__hoisted_51,
+              rows * (cols / 256U + (cols % 256U != 0U ? 1U : 0U)), 16U, 128U,
+              cols, gA, row_indices, gB, gC);
     MUST(cudaDeviceSynchronize());
 }
 
@@ -4983,8 +5106,10 @@ __hoisted_52(uint32_t cols,
              Kuiper_Sparse_Matrix_smatrix__float gA,
              uint32_t *row_indices, float *gB, float *gC)
 {
-    uint32_t m_idx = row_indices[blockIdx.x / ((cols + 255U) / 256U)];
-    uint32_t n_idx = blockIdx.x % ((cols + 255U) / 256U) * 256U;
+    uint32_t m_idx =
+        row_indices[blockIdx.x / (cols / 256U + (cols % 256U != 0U ? 1U : 0U))];
+    uint32_t n_idx =
+        blockIdx.x % (cols / 256U + (cols % 256U != 0U ? 1U : 0U)) * 256U;
     float *elems_tile = (float *)KPR_SHMEM_AT(0U);
     uint32_t *col_ind_tile = (uint32_t *) KPR_SHMEM_AT(128U);
     uint32_t ri = gA.row_off[m_idx];
@@ -5065,8 +5190,9 @@ Klas_SPMM_g_spmm_f32_256x32x16(uint32_t rows,
     KPR_SHMEM_FITS(256U);
     MUST(cudaFuncSetAttribute
          (__hoisted_52, cudaFuncAttributeMaxDynamicSharedMemorySize, 256U));
-    KPR_KCALL(__hoisted_52, rows * ((cols + 255U) / 256U), 16U, 256U, cols, gA,
-              row_indices, gB, gC);
+    KPR_KCALL(__hoisted_52,
+              rows * (cols / 256U + (cols % 256U != 0U ? 1U : 0U)), 16U, 256U,
+              cols, gA, row_indices, gB, gC);
     MUST(cudaDeviceSynchronize());
 }
 
@@ -5079,8 +5205,10 @@ __hoisted_53(uint32_t cols,
              Kuiper_Sparse_Matrix_smatrix__float gA,
              uint32_t *row_indices, float *gB, float *gC)
 {
-    uint32_t m_idx = row_indices[blockIdx.x / ((cols + 255U) / 256U)];
-    uint32_t n_idx = blockIdx.x % ((cols + 255U) / 256U) * 256U;
+    uint32_t m_idx =
+        row_indices[blockIdx.x / (cols / 256U + (cols % 256U != 0U ? 1U : 0U))];
+    uint32_t n_idx =
+        blockIdx.x % (cols / 256U + (cols % 256U != 0U ? 1U : 0U)) * 256U;
     float *elems_tile = (float *)KPR_SHMEM_AT(0U);
     uint32_t *col_ind_tile = (uint32_t *) KPR_SHMEM_AT(128U);
     uint32_t ri = gA.row_off[m_idx];
@@ -5161,8 +5289,9 @@ Klas_SPMM_g_spmm_f32_256x32x32(uint32_t rows,
     KPR_SHMEM_FITS(256U);
     MUST(cudaFuncSetAttribute
          (__hoisted_53, cudaFuncAttributeMaxDynamicSharedMemorySize, 256U));
-    KPR_KCALL(__hoisted_53, rows * ((cols + 255U) / 256U), 32U, 256U, cols, gA,
-              row_indices, gB, gC);
+    KPR_KCALL(__hoisted_53,
+              rows * (cols / 256U + (cols % 256U != 0U ? 1U : 0U)), 32U, 256U,
+              cols, gA, row_indices, gB, gC);
     MUST(cudaDeviceSynchronize());
 }
 
@@ -5175,8 +5304,10 @@ __hoisted_54(uint32_t cols,
              Kuiper_Sparse_Matrix_smatrix__float gA,
              uint32_t *row_indices, float *gB, float *gC)
 {
-    uint32_t m_idx = row_indices[blockIdx.x / ((cols + 255U) / 256U)];
-    uint32_t n_idx = blockIdx.x % ((cols + 255U) / 256U) * 256U;
+    uint32_t m_idx =
+        row_indices[blockIdx.x / (cols / 256U + (cols % 256U != 0U ? 1U : 0U))];
+    uint32_t n_idx =
+        blockIdx.x % (cols / 256U + (cols % 256U != 0U ? 1U : 0U)) * 256U;
     float *elems_tile = (float *)KPR_SHMEM_AT(0U);
     uint32_t *col_ind_tile = (uint32_t *) KPR_SHMEM_AT(256U);
     uint32_t ri = gA.row_off[m_idx];
@@ -5257,8 +5388,9 @@ Klas_SPMM_g_spmm_f32_256x64x16(uint32_t rows,
     KPR_SHMEM_FITS(512U);
     MUST(cudaFuncSetAttribute
          (__hoisted_54, cudaFuncAttributeMaxDynamicSharedMemorySize, 512U));
-    KPR_KCALL(__hoisted_54, rows * ((cols + 255U) / 256U), 16U, 512U, cols, gA,
-              row_indices, gB, gC);
+    KPR_KCALL(__hoisted_54,
+              rows * (cols / 256U + (cols % 256U != 0U ? 1U : 0U)), 16U, 512U,
+              cols, gA, row_indices, gB, gC);
     MUST(cudaDeviceSynchronize());
 }
 
@@ -5271,8 +5403,10 @@ __hoisted_55(uint32_t cols,
              Kuiper_Sparse_Matrix_smatrix__float gA,
              uint32_t *row_indices, float *gB, float *gC)
 {
-    uint32_t m_idx = row_indices[blockIdx.x / ((cols + 255U) / 256U)];
-    uint32_t n_idx = blockIdx.x % ((cols + 255U) / 256U) * 256U;
+    uint32_t m_idx =
+        row_indices[blockIdx.x / (cols / 256U + (cols % 256U != 0U ? 1U : 0U))];
+    uint32_t n_idx =
+        blockIdx.x % (cols / 256U + (cols % 256U != 0U ? 1U : 0U)) * 256U;
     float *elems_tile = (float *)KPR_SHMEM_AT(0U);
     uint32_t *col_ind_tile = (uint32_t *) KPR_SHMEM_AT(256U);
     uint32_t ri = gA.row_off[m_idx];
@@ -5353,8 +5487,9 @@ Klas_SPMM_g_spmm_f32_256x64x32(uint32_t rows,
     KPR_SHMEM_FITS(512U);
     MUST(cudaFuncSetAttribute
          (__hoisted_55, cudaFuncAttributeMaxDynamicSharedMemorySize, 512U));
-    KPR_KCALL(__hoisted_55, rows * ((cols + 255U) / 256U), 32U, 512U, cols, gA,
-              row_indices, gB, gC);
+    KPR_KCALL(__hoisted_55,
+              rows * (cols / 256U + (cols % 256U != 0U ? 1U : 0U)), 32U, 512U,
+              cols, gA, row_indices, gB, gC);
     MUST(cudaDeviceSynchronize());
 }
 
@@ -5367,8 +5502,10 @@ __hoisted_56(uint32_t cols,
              Kuiper_Sparse_Matrix_smatrix__float gA,
              uint32_t *row_indices, float *gB, float *gC)
 {
-    uint32_t m_idx = row_indices[blockIdx.x / ((cols + 255U) / 256U)];
-    uint32_t n_idx = blockIdx.x % ((cols + 255U) / 256U) * 256U;
+    uint32_t m_idx =
+        row_indices[blockIdx.x / (cols / 256U + (cols % 256U != 0U ? 1U : 0U))];
+    uint32_t n_idx =
+        blockIdx.x % (cols / 256U + (cols % 256U != 0U ? 1U : 0U)) * 256U;
     float *elems_tile = (float *)KPR_SHMEM_AT(0U);
     uint32_t *col_ind_tile = (uint32_t *) KPR_SHMEM_AT(256U);
     uint32_t ri = gA.row_off[m_idx];
@@ -5449,8 +5586,9 @@ Klas_SPMM_g_spmm_f32_256x64x64(uint32_t rows,
     KPR_SHMEM_FITS(512U);
     MUST(cudaFuncSetAttribute
          (__hoisted_56, cudaFuncAttributeMaxDynamicSharedMemorySize, 512U));
-    KPR_KCALL(__hoisted_56, rows * ((cols + 255U) / 256U), 64U, 512U, cols, gA,
-              row_indices, gB, gC);
+    KPR_KCALL(__hoisted_56,
+              rows * (cols / 256U + (cols % 256U != 0U ? 1U : 0U)), 64U, 512U,
+              cols, gA, row_indices, gB, gC);
     MUST(cudaDeviceSynchronize());
 }
 
@@ -5463,8 +5601,10 @@ __hoisted_57(uint32_t cols,
              Kuiper_Sparse_Matrix_smatrix__float gA,
              uint32_t *row_indices, float *gB, float *gC)
 {
-    uint32_t m_idx = row_indices[blockIdx.x / ((cols + 255U) / 256U)];
-    uint32_t n_idx = blockIdx.x % ((cols + 255U) / 256U) * 256U;
+    uint32_t m_idx =
+        row_indices[blockIdx.x / (cols / 256U + (cols % 256U != 0U ? 1U : 0U))];
+    uint32_t n_idx =
+        blockIdx.x % (cols / 256U + (cols % 256U != 0U ? 1U : 0U)) * 256U;
     float *elems_tile = (float *)KPR_SHMEM_AT(0U);
     uint32_t *col_ind_tile = (uint32_t *) KPR_SHMEM_AT(512U);
     uint32_t ri = gA.row_off[m_idx];
@@ -5545,8 +5685,9 @@ Klas_SPMM_g_spmm_f32_256x128x16(uint32_t rows,
     KPR_SHMEM_FITS(1024U);
     MUST(cudaFuncSetAttribute
          (__hoisted_57, cudaFuncAttributeMaxDynamicSharedMemorySize, 1024U));
-    KPR_KCALL(__hoisted_57, rows * ((cols + 255U) / 256U), 16U, 1024U, cols, gA,
-              row_indices, gB, gC);
+    KPR_KCALL(__hoisted_57,
+              rows * (cols / 256U + (cols % 256U != 0U ? 1U : 0U)), 16U, 1024U,
+              cols, gA, row_indices, gB, gC);
     MUST(cudaDeviceSynchronize());
 }
 
@@ -5559,8 +5700,10 @@ __hoisted_58(uint32_t cols,
              Kuiper_Sparse_Matrix_smatrix__float gA,
              uint32_t *row_indices, float *gB, float *gC)
 {
-    uint32_t m_idx = row_indices[blockIdx.x / ((cols + 255U) / 256U)];
-    uint32_t n_idx = blockIdx.x % ((cols + 255U) / 256U) * 256U;
+    uint32_t m_idx =
+        row_indices[blockIdx.x / (cols / 256U + (cols % 256U != 0U ? 1U : 0U))];
+    uint32_t n_idx =
+        blockIdx.x % (cols / 256U + (cols % 256U != 0U ? 1U : 0U)) * 256U;
     float *elems_tile = (float *)KPR_SHMEM_AT(0U);
     uint32_t *col_ind_tile = (uint32_t *) KPR_SHMEM_AT(512U);
     uint32_t ri = gA.row_off[m_idx];
@@ -5641,8 +5784,9 @@ Klas_SPMM_g_spmm_f32_256x128x32(uint32_t rows,
     KPR_SHMEM_FITS(1024U);
     MUST(cudaFuncSetAttribute
          (__hoisted_58, cudaFuncAttributeMaxDynamicSharedMemorySize, 1024U));
-    KPR_KCALL(__hoisted_58, rows * ((cols + 255U) / 256U), 32U, 1024U, cols, gA,
-              row_indices, gB, gC);
+    KPR_KCALL(__hoisted_58,
+              rows * (cols / 256U + (cols % 256U != 0U ? 1U : 0U)), 32U, 1024U,
+              cols, gA, row_indices, gB, gC);
     MUST(cudaDeviceSynchronize());
 }
 
@@ -5655,8 +5799,10 @@ __hoisted_59(uint32_t cols,
              Kuiper_Sparse_Matrix_smatrix__float gA,
              uint32_t *row_indices, float *gB, float *gC)
 {
-    uint32_t m_idx = row_indices[blockIdx.x / ((cols + 255U) / 256U)];
-    uint32_t n_idx = blockIdx.x % ((cols + 255U) / 256U) * 256U;
+    uint32_t m_idx =
+        row_indices[blockIdx.x / (cols / 256U + (cols % 256U != 0U ? 1U : 0U))];
+    uint32_t n_idx =
+        blockIdx.x % (cols / 256U + (cols % 256U != 0U ? 1U : 0U)) * 256U;
     float *elems_tile = (float *)KPR_SHMEM_AT(0U);
     uint32_t *col_ind_tile = (uint32_t *) KPR_SHMEM_AT(512U);
     uint32_t ri = gA.row_off[m_idx];
@@ -5737,8 +5883,9 @@ Klas_SPMM_g_spmm_f32_256x128x64(uint32_t rows,
     KPR_SHMEM_FITS(1024U);
     MUST(cudaFuncSetAttribute
          (__hoisted_59, cudaFuncAttributeMaxDynamicSharedMemorySize, 1024U));
-    KPR_KCALL(__hoisted_59, rows * ((cols + 255U) / 256U), 64U, 1024U, cols, gA,
-              row_indices, gB, gC);
+    KPR_KCALL(__hoisted_59,
+              rows * (cols / 256U + (cols % 256U != 0U ? 1U : 0U)), 64U, 1024U,
+              cols, gA, row_indices, gB, gC);
     MUST(cudaDeviceSynchronize());
 }
 
@@ -5751,8 +5898,10 @@ __hoisted_60(uint32_t cols,
              Kuiper_Sparse_Matrix_smatrix__float gA,
              uint32_t *row_indices, float *gB, float *gC)
 {
-    uint32_t m_idx = row_indices[blockIdx.x / ((cols + 255U) / 256U)];
-    uint32_t n_idx = blockIdx.x % ((cols + 255U) / 256U) * 256U;
+    uint32_t m_idx =
+        row_indices[blockIdx.x / (cols / 256U + (cols % 256U != 0U ? 1U : 0U))];
+    uint32_t n_idx =
+        blockIdx.x % (cols / 256U + (cols % 256U != 0U ? 1U : 0U)) * 256U;
     float *elems_tile = (float *)KPR_SHMEM_AT(0U);
     uint32_t *col_ind_tile = (uint32_t *) KPR_SHMEM_AT(512U);
     uint32_t ri = gA.row_off[m_idx];
@@ -5833,8 +5982,9 @@ Klas_SPMM_g_spmm_f32_256x128x128(uint32_t rows,
     KPR_SHMEM_FITS(1024U);
     MUST(cudaFuncSetAttribute
          (__hoisted_60, cudaFuncAttributeMaxDynamicSharedMemorySize, 1024U));
-    KPR_KCALL(__hoisted_60, rows * ((cols + 255U) / 256U), 128U, 1024U, cols,
-              gA, row_indices, gB, gC);
+    KPR_KCALL(__hoisted_60,
+              rows * (cols / 256U + (cols % 256U != 0U ? 1U : 0U)), 128U, 1024U,
+              cols, gA, row_indices, gB, gC);
     MUST(cudaDeviceSynchronize());
 }
 
@@ -5847,8 +5997,10 @@ __hoisted_61(uint32_t cols,
              Kuiper_Sparse_Matrix_smatrix__float gA,
              uint32_t *row_indices, float *gB, float *gC)
 {
-    uint32_t m_idx = row_indices[blockIdx.x / ((cols + 255U) / 256U)];
-    uint32_t n_idx = blockIdx.x % ((cols + 255U) / 256U) * 256U;
+    uint32_t m_idx =
+        row_indices[blockIdx.x / (cols / 256U + (cols % 256U != 0U ? 1U : 0U))];
+    uint32_t n_idx =
+        blockIdx.x % (cols / 256U + (cols % 256U != 0U ? 1U : 0U)) * 256U;
     float *elems_tile = (float *)KPR_SHMEM_AT(0U);
     uint32_t *col_ind_tile = (uint32_t *) KPR_SHMEM_AT(1024U);
     uint32_t ri = gA.row_off[m_idx];
@@ -5929,8 +6081,9 @@ Klas_SPMM_g_spmm_f32_256x256x16(uint32_t rows,
     KPR_SHMEM_FITS(2048U);
     MUST(cudaFuncSetAttribute
          (__hoisted_61, cudaFuncAttributeMaxDynamicSharedMemorySize, 2048U));
-    KPR_KCALL(__hoisted_61, rows * ((cols + 255U) / 256U), 16U, 2048U, cols, gA,
-              row_indices, gB, gC);
+    KPR_KCALL(__hoisted_61,
+              rows * (cols / 256U + (cols % 256U != 0U ? 1U : 0U)), 16U, 2048U,
+              cols, gA, row_indices, gB, gC);
     MUST(cudaDeviceSynchronize());
 }
 
@@ -5943,8 +6096,10 @@ __hoisted_62(uint32_t cols,
              Kuiper_Sparse_Matrix_smatrix__float gA,
              uint32_t *row_indices, float *gB, float *gC)
 {
-    uint32_t m_idx = row_indices[blockIdx.x / ((cols + 255U) / 256U)];
-    uint32_t n_idx = blockIdx.x % ((cols + 255U) / 256U) * 256U;
+    uint32_t m_idx =
+        row_indices[blockIdx.x / (cols / 256U + (cols % 256U != 0U ? 1U : 0U))];
+    uint32_t n_idx =
+        blockIdx.x % (cols / 256U + (cols % 256U != 0U ? 1U : 0U)) * 256U;
     float *elems_tile = (float *)KPR_SHMEM_AT(0U);
     uint32_t *col_ind_tile = (uint32_t *) KPR_SHMEM_AT(1024U);
     uint32_t ri = gA.row_off[m_idx];
@@ -6025,8 +6180,9 @@ Klas_SPMM_g_spmm_f32_256x256x32(uint32_t rows,
     KPR_SHMEM_FITS(2048U);
     MUST(cudaFuncSetAttribute
          (__hoisted_62, cudaFuncAttributeMaxDynamicSharedMemorySize, 2048U));
-    KPR_KCALL(__hoisted_62, rows * ((cols + 255U) / 256U), 32U, 2048U, cols, gA,
-              row_indices, gB, gC);
+    KPR_KCALL(__hoisted_62,
+              rows * (cols / 256U + (cols % 256U != 0U ? 1U : 0U)), 32U, 2048U,
+              cols, gA, row_indices, gB, gC);
     MUST(cudaDeviceSynchronize());
 }
 
@@ -6039,8 +6195,10 @@ __hoisted_63(uint32_t cols,
              Kuiper_Sparse_Matrix_smatrix__float gA,
              uint32_t *row_indices, float *gB, float *gC)
 {
-    uint32_t m_idx = row_indices[blockIdx.x / ((cols + 255U) / 256U)];
-    uint32_t n_idx = blockIdx.x % ((cols + 255U) / 256U) * 256U;
+    uint32_t m_idx =
+        row_indices[blockIdx.x / (cols / 256U + (cols % 256U != 0U ? 1U : 0U))];
+    uint32_t n_idx =
+        blockIdx.x % (cols / 256U + (cols % 256U != 0U ? 1U : 0U)) * 256U;
     float *elems_tile = (float *)KPR_SHMEM_AT(0U);
     uint32_t *col_ind_tile = (uint32_t *) KPR_SHMEM_AT(1024U);
     uint32_t ri = gA.row_off[m_idx];
@@ -6121,8 +6279,9 @@ Klas_SPMM_g_spmm_f32_256x256x64(uint32_t rows,
     KPR_SHMEM_FITS(2048U);
     MUST(cudaFuncSetAttribute
          (__hoisted_63, cudaFuncAttributeMaxDynamicSharedMemorySize, 2048U));
-    KPR_KCALL(__hoisted_63, rows * ((cols + 255U) / 256U), 64U, 2048U, cols, gA,
-              row_indices, gB, gC);
+    KPR_KCALL(__hoisted_63,
+              rows * (cols / 256U + (cols % 256U != 0U ? 1U : 0U)), 64U, 2048U,
+              cols, gA, row_indices, gB, gC);
     MUST(cudaDeviceSynchronize());
 }
 
@@ -6135,8 +6294,10 @@ __hoisted_64(uint32_t cols,
              Kuiper_Sparse_Matrix_smatrix__float gA,
              uint32_t *row_indices, float *gB, float *gC)
 {
-    uint32_t m_idx = row_indices[blockIdx.x / ((cols + 255U) / 256U)];
-    uint32_t n_idx = blockIdx.x % ((cols + 255U) / 256U) * 256U;
+    uint32_t m_idx =
+        row_indices[blockIdx.x / (cols / 256U + (cols % 256U != 0U ? 1U : 0U))];
+    uint32_t n_idx =
+        blockIdx.x % (cols / 256U + (cols % 256U != 0U ? 1U : 0U)) * 256U;
     float *elems_tile = (float *)KPR_SHMEM_AT(0U);
     uint32_t *col_ind_tile = (uint32_t *) KPR_SHMEM_AT(1024U);
     uint32_t ri = gA.row_off[m_idx];
@@ -6217,8 +6378,9 @@ Klas_SPMM_g_spmm_f32_256x256x128(uint32_t rows,
     KPR_SHMEM_FITS(2048U);
     MUST(cudaFuncSetAttribute
          (__hoisted_64, cudaFuncAttributeMaxDynamicSharedMemorySize, 2048U));
-    KPR_KCALL(__hoisted_64, rows * ((cols + 255U) / 256U), 128U, 2048U, cols,
-              gA, row_indices, gB, gC);
+    KPR_KCALL(__hoisted_64,
+              rows * (cols / 256U + (cols % 256U != 0U ? 1U : 0U)), 128U, 2048U,
+              cols, gA, row_indices, gB, gC);
     MUST(cudaDeviceSynchronize());
 }
 
@@ -6231,8 +6393,10 @@ __hoisted_65(uint32_t cols,
              Kuiper_Sparse_Matrix_smatrix__float gA,
              uint32_t *row_indices, float *gB, float *gC)
 {
-    uint32_t m_idx = row_indices[blockIdx.x / ((cols + 255U) / 256U)];
-    uint32_t n_idx = blockIdx.x % ((cols + 255U) / 256U) * 256U;
+    uint32_t m_idx =
+        row_indices[blockIdx.x / (cols / 256U + (cols % 256U != 0U ? 1U : 0U))];
+    uint32_t n_idx =
+        blockIdx.x % (cols / 256U + (cols % 256U != 0U ? 1U : 0U)) * 256U;
     float *elems_tile = (float *)KPR_SHMEM_AT(0U);
     uint32_t *col_ind_tile = (uint32_t *) KPR_SHMEM_AT(1024U);
     uint32_t ri = gA.row_off[m_idx];
@@ -6312,8 +6476,9 @@ Klas_SPMM_g_spmm_f32_256x256x256(uint32_t rows,
     KPR_SHMEM_FITS(2048U);
     MUST(cudaFuncSetAttribute
          (__hoisted_65, cudaFuncAttributeMaxDynamicSharedMemorySize, 2048U));
-    KPR_KCALL(__hoisted_65, rows * ((cols + 255U) / 256U), 256U, 2048U, cols,
-              gA, row_indices, gB, gC);
+    KPR_KCALL(__hoisted_65,
+              rows * (cols / 256U + (cols % 256U != 0U ? 1U : 0U)), 256U, 2048U,
+              cols, gA, row_indices, gB, gC);
     MUST(cudaDeviceSynchronize());
 }
 
@@ -6326,8 +6491,10 @@ __hoisted_66(uint32_t cols,
              Kuiper_Sparse_Matrix_smatrix__float gA,
              uint32_t *row_indices, float *gB, float *gC)
 {
-    uint32_t m_idx = row_indices[blockIdx.x / ((cols + 255U) / 256U)];
-    uint32_t n_idx = blockIdx.x % ((cols + 255U) / 256U) * 256U;
+    uint32_t m_idx =
+        row_indices[blockIdx.x / (cols / 256U + (cols % 256U != 0U ? 1U : 0U))];
+    uint32_t n_idx =
+        blockIdx.x % (cols / 256U + (cols % 256U != 0U ? 1U : 0U)) * 256U;
     float *elems_tile = (float *)KPR_SHMEM_AT(0U);
     uint32_t *col_ind_tile = (uint32_t *) KPR_SHMEM_AT(2048U);
     uint32_t ri = gA.row_off[m_idx];
@@ -6408,8 +6575,9 @@ Klas_SPMM_g_spmm_f32_256x512x16(uint32_t rows,
     KPR_SHMEM_FITS(4096U);
     MUST(cudaFuncSetAttribute
          (__hoisted_66, cudaFuncAttributeMaxDynamicSharedMemorySize, 4096U));
-    KPR_KCALL(__hoisted_66, rows * ((cols + 255U) / 256U), 16U, 4096U, cols, gA,
-              row_indices, gB, gC);
+    KPR_KCALL(__hoisted_66,
+              rows * (cols / 256U + (cols % 256U != 0U ? 1U : 0U)), 16U, 4096U,
+              cols, gA, row_indices, gB, gC);
     MUST(cudaDeviceSynchronize());
 }
 
@@ -6422,8 +6590,10 @@ __hoisted_67(uint32_t cols,
              Kuiper_Sparse_Matrix_smatrix__float gA,
              uint32_t *row_indices, float *gB, float *gC)
 {
-    uint32_t m_idx = row_indices[blockIdx.x / ((cols + 255U) / 256U)];
-    uint32_t n_idx = blockIdx.x % ((cols + 255U) / 256U) * 256U;
+    uint32_t m_idx =
+        row_indices[blockIdx.x / (cols / 256U + (cols % 256U != 0U ? 1U : 0U))];
+    uint32_t n_idx =
+        blockIdx.x % (cols / 256U + (cols % 256U != 0U ? 1U : 0U)) * 256U;
     float *elems_tile = (float *)KPR_SHMEM_AT(0U);
     uint32_t *col_ind_tile = (uint32_t *) KPR_SHMEM_AT(2048U);
     uint32_t ri = gA.row_off[m_idx];
@@ -6504,8 +6674,9 @@ Klas_SPMM_g_spmm_f32_256x512x32(uint32_t rows,
     KPR_SHMEM_FITS(4096U);
     MUST(cudaFuncSetAttribute
          (__hoisted_67, cudaFuncAttributeMaxDynamicSharedMemorySize, 4096U));
-    KPR_KCALL(__hoisted_67, rows * ((cols + 255U) / 256U), 32U, 4096U, cols, gA,
-              row_indices, gB, gC);
+    KPR_KCALL(__hoisted_67,
+              rows * (cols / 256U + (cols % 256U != 0U ? 1U : 0U)), 32U, 4096U,
+              cols, gA, row_indices, gB, gC);
     MUST(cudaDeviceSynchronize());
 }
 
@@ -6518,8 +6689,10 @@ __hoisted_68(uint32_t cols,
              Kuiper_Sparse_Matrix_smatrix__float gA,
              uint32_t *row_indices, float *gB, float *gC)
 {
-    uint32_t m_idx = row_indices[blockIdx.x / ((cols + 255U) / 256U)];
-    uint32_t n_idx = blockIdx.x % ((cols + 255U) / 256U) * 256U;
+    uint32_t m_idx =
+        row_indices[blockIdx.x / (cols / 256U + (cols % 256U != 0U ? 1U : 0U))];
+    uint32_t n_idx =
+        blockIdx.x % (cols / 256U + (cols % 256U != 0U ? 1U : 0U)) * 256U;
     float *elems_tile = (float *)KPR_SHMEM_AT(0U);
     uint32_t *col_ind_tile = (uint32_t *) KPR_SHMEM_AT(2048U);
     uint32_t ri = gA.row_off[m_idx];
@@ -6600,8 +6773,9 @@ Klas_SPMM_g_spmm_f32_256x512x64(uint32_t rows,
     KPR_SHMEM_FITS(4096U);
     MUST(cudaFuncSetAttribute
          (__hoisted_68, cudaFuncAttributeMaxDynamicSharedMemorySize, 4096U));
-    KPR_KCALL(__hoisted_68, rows * ((cols + 255U) / 256U), 64U, 4096U, cols, gA,
-              row_indices, gB, gC);
+    KPR_KCALL(__hoisted_68,
+              rows * (cols / 256U + (cols % 256U != 0U ? 1U : 0U)), 64U, 4096U,
+              cols, gA, row_indices, gB, gC);
     MUST(cudaDeviceSynchronize());
 }
 
@@ -6614,8 +6788,10 @@ __hoisted_69(uint32_t cols,
              Kuiper_Sparse_Matrix_smatrix__float gA,
              uint32_t *row_indices, float *gB, float *gC)
 {
-    uint32_t m_idx = row_indices[blockIdx.x / ((cols + 255U) / 256U)];
-    uint32_t n_idx = blockIdx.x % ((cols + 255U) / 256U) * 256U;
+    uint32_t m_idx =
+        row_indices[blockIdx.x / (cols / 256U + (cols % 256U != 0U ? 1U : 0U))];
+    uint32_t n_idx =
+        blockIdx.x % (cols / 256U + (cols % 256U != 0U ? 1U : 0U)) * 256U;
     float *elems_tile = (float *)KPR_SHMEM_AT(0U);
     uint32_t *col_ind_tile = (uint32_t *) KPR_SHMEM_AT(2048U);
     uint32_t ri = gA.row_off[m_idx];
@@ -6696,8 +6872,9 @@ Klas_SPMM_g_spmm_f32_256x512x128(uint32_t rows,
     KPR_SHMEM_FITS(4096U);
     MUST(cudaFuncSetAttribute
          (__hoisted_69, cudaFuncAttributeMaxDynamicSharedMemorySize, 4096U));
-    KPR_KCALL(__hoisted_69, rows * ((cols + 255U) / 256U), 128U, 4096U, cols,
-              gA, row_indices, gB, gC);
+    KPR_KCALL(__hoisted_69,
+              rows * (cols / 256U + (cols % 256U != 0U ? 1U : 0U)), 128U, 4096U,
+              cols, gA, row_indices, gB, gC);
     MUST(cudaDeviceSynchronize());
 }
 
@@ -6710,8 +6887,10 @@ __hoisted_70(uint32_t cols,
              Kuiper_Sparse_Matrix_smatrix__float gA,
              uint32_t *row_indices, float *gB, float *gC)
 {
-    uint32_t m_idx = row_indices[blockIdx.x / ((cols + 255U) / 256U)];
-    uint32_t n_idx = blockIdx.x % ((cols + 255U) / 256U) * 256U;
+    uint32_t m_idx =
+        row_indices[blockIdx.x / (cols / 256U + (cols % 256U != 0U ? 1U : 0U))];
+    uint32_t n_idx =
+        blockIdx.x % (cols / 256U + (cols % 256U != 0U ? 1U : 0U)) * 256U;
     float *elems_tile = (float *)KPR_SHMEM_AT(0U);
     uint32_t *col_ind_tile = (uint32_t *) KPR_SHMEM_AT(2048U);
     uint32_t ri = gA.row_off[m_idx];
@@ -6791,8 +6970,9 @@ Klas_SPMM_g_spmm_f32_256x512x256(uint32_t rows,
     KPR_SHMEM_FITS(4096U);
     MUST(cudaFuncSetAttribute
          (__hoisted_70, cudaFuncAttributeMaxDynamicSharedMemorySize, 4096U));
-    KPR_KCALL(__hoisted_70, rows * ((cols + 255U) / 256U), 256U, 4096U, cols,
-              gA, row_indices, gB, gC);
+    KPR_KCALL(__hoisted_70,
+              rows * (cols / 256U + (cols % 256U != 0U ? 1U : 0U)), 256U, 4096U,
+              cols, gA, row_indices, gB, gC);
     MUST(cudaDeviceSynchronize());
 }
 
@@ -6805,8 +6985,10 @@ __hoisted_71(uint32_t cols,
              Kuiper_Sparse_Matrix_smatrix__float gA,
              uint32_t *row_indices, float *gB, float *gC)
 {
-    uint32_t m_idx = row_indices[blockIdx.x / ((cols + 511U) / 512U)];
-    uint32_t n_idx = blockIdx.x % ((cols + 511U) / 512U) * 512U;
+    uint32_t m_idx =
+        row_indices[blockIdx.x / (cols / 512U + (cols % 512U != 0U ? 1U : 0U))];
+    uint32_t n_idx =
+        blockIdx.x % (cols / 512U + (cols % 512U != 0U ? 1U : 0U)) * 512U;
     float *elems_tile = (float *)KPR_SHMEM_AT(0U);
     uint32_t *col_ind_tile = (uint32_t *) KPR_SHMEM_AT(64U);
     uint32_t ri = gA.row_off[m_idx];
@@ -6887,8 +7069,9 @@ Klas_SPMM_g_spmm_f32_512x16x16(uint32_t rows,
     KPR_SHMEM_FITS(128U);
     MUST(cudaFuncSetAttribute
          (__hoisted_71, cudaFuncAttributeMaxDynamicSharedMemorySize, 128U));
-    KPR_KCALL(__hoisted_71, rows * ((cols + 511U) / 512U), 16U, 128U, cols, gA,
-              row_indices, gB, gC);
+    KPR_KCALL(__hoisted_71,
+              rows * (cols / 512U + (cols % 512U != 0U ? 1U : 0U)), 16U, 128U,
+              cols, gA, row_indices, gB, gC);
     MUST(cudaDeviceSynchronize());
 }
 
@@ -6901,8 +7084,10 @@ __hoisted_72(uint32_t cols,
              Kuiper_Sparse_Matrix_smatrix__float gA,
              uint32_t *row_indices, float *gB, float *gC)
 {
-    uint32_t m_idx = row_indices[blockIdx.x / ((cols + 511U) / 512U)];
-    uint32_t n_idx = blockIdx.x % ((cols + 511U) / 512U) * 512U;
+    uint32_t m_idx =
+        row_indices[blockIdx.x / (cols / 512U + (cols % 512U != 0U ? 1U : 0U))];
+    uint32_t n_idx =
+        blockIdx.x % (cols / 512U + (cols % 512U != 0U ? 1U : 0U)) * 512U;
     float *elems_tile = (float *)KPR_SHMEM_AT(0U);
     uint32_t *col_ind_tile = (uint32_t *) KPR_SHMEM_AT(128U);
     uint32_t ri = gA.row_off[m_idx];
@@ -6983,8 +7168,9 @@ Klas_SPMM_g_spmm_f32_512x32x16(uint32_t rows,
     KPR_SHMEM_FITS(256U);
     MUST(cudaFuncSetAttribute
          (__hoisted_72, cudaFuncAttributeMaxDynamicSharedMemorySize, 256U));
-    KPR_KCALL(__hoisted_72, rows * ((cols + 511U) / 512U), 16U, 256U, cols, gA,
-              row_indices, gB, gC);
+    KPR_KCALL(__hoisted_72,
+              rows * (cols / 512U + (cols % 512U != 0U ? 1U : 0U)), 16U, 256U,
+              cols, gA, row_indices, gB, gC);
     MUST(cudaDeviceSynchronize());
 }
 
@@ -6997,8 +7183,10 @@ __hoisted_73(uint32_t cols,
              Kuiper_Sparse_Matrix_smatrix__float gA,
              uint32_t *row_indices, float *gB, float *gC)
 {
-    uint32_t m_idx = row_indices[blockIdx.x / ((cols + 511U) / 512U)];
-    uint32_t n_idx = blockIdx.x % ((cols + 511U) / 512U) * 512U;
+    uint32_t m_idx =
+        row_indices[blockIdx.x / (cols / 512U + (cols % 512U != 0U ? 1U : 0U))];
+    uint32_t n_idx =
+        blockIdx.x % (cols / 512U + (cols % 512U != 0U ? 1U : 0U)) * 512U;
     float *elems_tile = (float *)KPR_SHMEM_AT(0U);
     uint32_t *col_ind_tile = (uint32_t *) KPR_SHMEM_AT(128U);
     uint32_t ri = gA.row_off[m_idx];
@@ -7079,8 +7267,9 @@ Klas_SPMM_g_spmm_f32_512x32x32(uint32_t rows,
     KPR_SHMEM_FITS(256U);
     MUST(cudaFuncSetAttribute
          (__hoisted_73, cudaFuncAttributeMaxDynamicSharedMemorySize, 256U));
-    KPR_KCALL(__hoisted_73, rows * ((cols + 511U) / 512U), 32U, 256U, cols, gA,
-              row_indices, gB, gC);
+    KPR_KCALL(__hoisted_73,
+              rows * (cols / 512U + (cols % 512U != 0U ? 1U : 0U)), 32U, 256U,
+              cols, gA, row_indices, gB, gC);
     MUST(cudaDeviceSynchronize());
 }
 
@@ -7093,8 +7282,10 @@ __hoisted_74(uint32_t cols,
              Kuiper_Sparse_Matrix_smatrix__float gA,
              uint32_t *row_indices, float *gB, float *gC)
 {
-    uint32_t m_idx = row_indices[blockIdx.x / ((cols + 511U) / 512U)];
-    uint32_t n_idx = blockIdx.x % ((cols + 511U) / 512U) * 512U;
+    uint32_t m_idx =
+        row_indices[blockIdx.x / (cols / 512U + (cols % 512U != 0U ? 1U : 0U))];
+    uint32_t n_idx =
+        blockIdx.x % (cols / 512U + (cols % 512U != 0U ? 1U : 0U)) * 512U;
     float *elems_tile = (float *)KPR_SHMEM_AT(0U);
     uint32_t *col_ind_tile = (uint32_t *) KPR_SHMEM_AT(256U);
     uint32_t ri = gA.row_off[m_idx];
@@ -7175,8 +7366,9 @@ Klas_SPMM_g_spmm_f32_512x64x16(uint32_t rows,
     KPR_SHMEM_FITS(512U);
     MUST(cudaFuncSetAttribute
          (__hoisted_74, cudaFuncAttributeMaxDynamicSharedMemorySize, 512U));
-    KPR_KCALL(__hoisted_74, rows * ((cols + 511U) / 512U), 16U, 512U, cols, gA,
-              row_indices, gB, gC);
+    KPR_KCALL(__hoisted_74,
+              rows * (cols / 512U + (cols % 512U != 0U ? 1U : 0U)), 16U, 512U,
+              cols, gA, row_indices, gB, gC);
     MUST(cudaDeviceSynchronize());
 }
 
@@ -7189,8 +7381,10 @@ __hoisted_75(uint32_t cols,
              Kuiper_Sparse_Matrix_smatrix__float gA,
              uint32_t *row_indices, float *gB, float *gC)
 {
-    uint32_t m_idx = row_indices[blockIdx.x / ((cols + 511U) / 512U)];
-    uint32_t n_idx = blockIdx.x % ((cols + 511U) / 512U) * 512U;
+    uint32_t m_idx =
+        row_indices[blockIdx.x / (cols / 512U + (cols % 512U != 0U ? 1U : 0U))];
+    uint32_t n_idx =
+        blockIdx.x % (cols / 512U + (cols % 512U != 0U ? 1U : 0U)) * 512U;
     float *elems_tile = (float *)KPR_SHMEM_AT(0U);
     uint32_t *col_ind_tile = (uint32_t *) KPR_SHMEM_AT(256U);
     uint32_t ri = gA.row_off[m_idx];
@@ -7271,8 +7465,9 @@ Klas_SPMM_g_spmm_f32_512x64x32(uint32_t rows,
     KPR_SHMEM_FITS(512U);
     MUST(cudaFuncSetAttribute
          (__hoisted_75, cudaFuncAttributeMaxDynamicSharedMemorySize, 512U));
-    KPR_KCALL(__hoisted_75, rows * ((cols + 511U) / 512U), 32U, 512U, cols, gA,
-              row_indices, gB, gC);
+    KPR_KCALL(__hoisted_75,
+              rows * (cols / 512U + (cols % 512U != 0U ? 1U : 0U)), 32U, 512U,
+              cols, gA, row_indices, gB, gC);
     MUST(cudaDeviceSynchronize());
 }
 
@@ -7285,8 +7480,10 @@ __hoisted_76(uint32_t cols,
              Kuiper_Sparse_Matrix_smatrix__float gA,
              uint32_t *row_indices, float *gB, float *gC)
 {
-    uint32_t m_idx = row_indices[blockIdx.x / ((cols + 511U) / 512U)];
-    uint32_t n_idx = blockIdx.x % ((cols + 511U) / 512U) * 512U;
+    uint32_t m_idx =
+        row_indices[blockIdx.x / (cols / 512U + (cols % 512U != 0U ? 1U : 0U))];
+    uint32_t n_idx =
+        blockIdx.x % (cols / 512U + (cols % 512U != 0U ? 1U : 0U)) * 512U;
     float *elems_tile = (float *)KPR_SHMEM_AT(0U);
     uint32_t *col_ind_tile = (uint32_t *) KPR_SHMEM_AT(256U);
     uint32_t ri = gA.row_off[m_idx];
@@ -7367,8 +7564,9 @@ Klas_SPMM_g_spmm_f32_512x64x64(uint32_t rows,
     KPR_SHMEM_FITS(512U);
     MUST(cudaFuncSetAttribute
          (__hoisted_76, cudaFuncAttributeMaxDynamicSharedMemorySize, 512U));
-    KPR_KCALL(__hoisted_76, rows * ((cols + 511U) / 512U), 64U, 512U, cols, gA,
-              row_indices, gB, gC);
+    KPR_KCALL(__hoisted_76,
+              rows * (cols / 512U + (cols % 512U != 0U ? 1U : 0U)), 64U, 512U,
+              cols, gA, row_indices, gB, gC);
     MUST(cudaDeviceSynchronize());
 }
 
@@ -7381,8 +7579,10 @@ __hoisted_77(uint32_t cols,
              Kuiper_Sparse_Matrix_smatrix__float gA,
              uint32_t *row_indices, float *gB, float *gC)
 {
-    uint32_t m_idx = row_indices[blockIdx.x / ((cols + 511U) / 512U)];
-    uint32_t n_idx = blockIdx.x % ((cols + 511U) / 512U) * 512U;
+    uint32_t m_idx =
+        row_indices[blockIdx.x / (cols / 512U + (cols % 512U != 0U ? 1U : 0U))];
+    uint32_t n_idx =
+        blockIdx.x % (cols / 512U + (cols % 512U != 0U ? 1U : 0U)) * 512U;
     float *elems_tile = (float *)KPR_SHMEM_AT(0U);
     uint32_t *col_ind_tile = (uint32_t *) KPR_SHMEM_AT(512U);
     uint32_t ri = gA.row_off[m_idx];
@@ -7463,8 +7663,9 @@ Klas_SPMM_g_spmm_f32_512x128x16(uint32_t rows,
     KPR_SHMEM_FITS(1024U);
     MUST(cudaFuncSetAttribute
          (__hoisted_77, cudaFuncAttributeMaxDynamicSharedMemorySize, 1024U));
-    KPR_KCALL(__hoisted_77, rows * ((cols + 511U) / 512U), 16U, 1024U, cols, gA,
-              row_indices, gB, gC);
+    KPR_KCALL(__hoisted_77,
+              rows * (cols / 512U + (cols % 512U != 0U ? 1U : 0U)), 16U, 1024U,
+              cols, gA, row_indices, gB, gC);
     MUST(cudaDeviceSynchronize());
 }
 
@@ -7477,8 +7678,10 @@ __hoisted_78(uint32_t cols,
              Kuiper_Sparse_Matrix_smatrix__float gA,
              uint32_t *row_indices, float *gB, float *gC)
 {
-    uint32_t m_idx = row_indices[blockIdx.x / ((cols + 511U) / 512U)];
-    uint32_t n_idx = blockIdx.x % ((cols + 511U) / 512U) * 512U;
+    uint32_t m_idx =
+        row_indices[blockIdx.x / (cols / 512U + (cols % 512U != 0U ? 1U : 0U))];
+    uint32_t n_idx =
+        blockIdx.x % (cols / 512U + (cols % 512U != 0U ? 1U : 0U)) * 512U;
     float *elems_tile = (float *)KPR_SHMEM_AT(0U);
     uint32_t *col_ind_tile = (uint32_t *) KPR_SHMEM_AT(512U);
     uint32_t ri = gA.row_off[m_idx];
@@ -7559,8 +7762,9 @@ Klas_SPMM_g_spmm_f32_512x128x32(uint32_t rows,
     KPR_SHMEM_FITS(1024U);
     MUST(cudaFuncSetAttribute
          (__hoisted_78, cudaFuncAttributeMaxDynamicSharedMemorySize, 1024U));
-    KPR_KCALL(__hoisted_78, rows * ((cols + 511U) / 512U), 32U, 1024U, cols, gA,
-              row_indices, gB, gC);
+    KPR_KCALL(__hoisted_78,
+              rows * (cols / 512U + (cols % 512U != 0U ? 1U : 0U)), 32U, 1024U,
+              cols, gA, row_indices, gB, gC);
     MUST(cudaDeviceSynchronize());
 }
 
@@ -7573,8 +7777,10 @@ __hoisted_79(uint32_t cols,
              Kuiper_Sparse_Matrix_smatrix__float gA,
              uint32_t *row_indices, float *gB, float *gC)
 {
-    uint32_t m_idx = row_indices[blockIdx.x / ((cols + 511U) / 512U)];
-    uint32_t n_idx = blockIdx.x % ((cols + 511U) / 512U) * 512U;
+    uint32_t m_idx =
+        row_indices[blockIdx.x / (cols / 512U + (cols % 512U != 0U ? 1U : 0U))];
+    uint32_t n_idx =
+        blockIdx.x % (cols / 512U + (cols % 512U != 0U ? 1U : 0U)) * 512U;
     float *elems_tile = (float *)KPR_SHMEM_AT(0U);
     uint32_t *col_ind_tile = (uint32_t *) KPR_SHMEM_AT(512U);
     uint32_t ri = gA.row_off[m_idx];
@@ -7655,8 +7861,9 @@ Klas_SPMM_g_spmm_f32_512x128x64(uint32_t rows,
     KPR_SHMEM_FITS(1024U);
     MUST(cudaFuncSetAttribute
          (__hoisted_79, cudaFuncAttributeMaxDynamicSharedMemorySize, 1024U));
-    KPR_KCALL(__hoisted_79, rows * ((cols + 511U) / 512U), 64U, 1024U, cols, gA,
-              row_indices, gB, gC);
+    KPR_KCALL(__hoisted_79,
+              rows * (cols / 512U + (cols % 512U != 0U ? 1U : 0U)), 64U, 1024U,
+              cols, gA, row_indices, gB, gC);
     MUST(cudaDeviceSynchronize());
 }
 
@@ -7669,8 +7876,10 @@ __hoisted_80(uint32_t cols,
              Kuiper_Sparse_Matrix_smatrix__float gA,
              uint32_t *row_indices, float *gB, float *gC)
 {
-    uint32_t m_idx = row_indices[blockIdx.x / ((cols + 511U) / 512U)];
-    uint32_t n_idx = blockIdx.x % ((cols + 511U) / 512U) * 512U;
+    uint32_t m_idx =
+        row_indices[blockIdx.x / (cols / 512U + (cols % 512U != 0U ? 1U : 0U))];
+    uint32_t n_idx =
+        blockIdx.x % (cols / 512U + (cols % 512U != 0U ? 1U : 0U)) * 512U;
     float *elems_tile = (float *)KPR_SHMEM_AT(0U);
     uint32_t *col_ind_tile = (uint32_t *) KPR_SHMEM_AT(512U);
     uint32_t ri = gA.row_off[m_idx];
@@ -7751,8 +7960,9 @@ Klas_SPMM_g_spmm_f32_512x128x128(uint32_t rows,
     KPR_SHMEM_FITS(1024U);
     MUST(cudaFuncSetAttribute
          (__hoisted_80, cudaFuncAttributeMaxDynamicSharedMemorySize, 1024U));
-    KPR_KCALL(__hoisted_80, rows * ((cols + 511U) / 512U), 128U, 1024U, cols,
-              gA, row_indices, gB, gC);
+    KPR_KCALL(__hoisted_80,
+              rows * (cols / 512U + (cols % 512U != 0U ? 1U : 0U)), 128U, 1024U,
+              cols, gA, row_indices, gB, gC);
     MUST(cudaDeviceSynchronize());
 }
 
@@ -7765,8 +7975,10 @@ __hoisted_81(uint32_t cols,
              Kuiper_Sparse_Matrix_smatrix__float gA,
              uint32_t *row_indices, float *gB, float *gC)
 {
-    uint32_t m_idx = row_indices[blockIdx.x / ((cols + 511U) / 512U)];
-    uint32_t n_idx = blockIdx.x % ((cols + 511U) / 512U) * 512U;
+    uint32_t m_idx =
+        row_indices[blockIdx.x / (cols / 512U + (cols % 512U != 0U ? 1U : 0U))];
+    uint32_t n_idx =
+        blockIdx.x % (cols / 512U + (cols % 512U != 0U ? 1U : 0U)) * 512U;
     float *elems_tile = (float *)KPR_SHMEM_AT(0U);
     uint32_t *col_ind_tile = (uint32_t *) KPR_SHMEM_AT(1024U);
     uint32_t ri = gA.row_off[m_idx];
@@ -7847,8 +8059,9 @@ Klas_SPMM_g_spmm_f32_512x256x16(uint32_t rows,
     KPR_SHMEM_FITS(2048U);
     MUST(cudaFuncSetAttribute
          (__hoisted_81, cudaFuncAttributeMaxDynamicSharedMemorySize, 2048U));
-    KPR_KCALL(__hoisted_81, rows * ((cols + 511U) / 512U), 16U, 2048U, cols, gA,
-              row_indices, gB, gC);
+    KPR_KCALL(__hoisted_81,
+              rows * (cols / 512U + (cols % 512U != 0U ? 1U : 0U)), 16U, 2048U,
+              cols, gA, row_indices, gB, gC);
     MUST(cudaDeviceSynchronize());
 }
 
@@ -7861,8 +8074,10 @@ __hoisted_82(uint32_t cols,
              Kuiper_Sparse_Matrix_smatrix__float gA,
              uint32_t *row_indices, float *gB, float *gC)
 {
-    uint32_t m_idx = row_indices[blockIdx.x / ((cols + 511U) / 512U)];
-    uint32_t n_idx = blockIdx.x % ((cols + 511U) / 512U) * 512U;
+    uint32_t m_idx =
+        row_indices[blockIdx.x / (cols / 512U + (cols % 512U != 0U ? 1U : 0U))];
+    uint32_t n_idx =
+        blockIdx.x % (cols / 512U + (cols % 512U != 0U ? 1U : 0U)) * 512U;
     float *elems_tile = (float *)KPR_SHMEM_AT(0U);
     uint32_t *col_ind_tile = (uint32_t *) KPR_SHMEM_AT(1024U);
     uint32_t ri = gA.row_off[m_idx];
@@ -7943,8 +8158,9 @@ Klas_SPMM_g_spmm_f32_512x256x32(uint32_t rows,
     KPR_SHMEM_FITS(2048U);
     MUST(cudaFuncSetAttribute
          (__hoisted_82, cudaFuncAttributeMaxDynamicSharedMemorySize, 2048U));
-    KPR_KCALL(__hoisted_82, rows * ((cols + 511U) / 512U), 32U, 2048U, cols, gA,
-              row_indices, gB, gC);
+    KPR_KCALL(__hoisted_82,
+              rows * (cols / 512U + (cols % 512U != 0U ? 1U : 0U)), 32U, 2048U,
+              cols, gA, row_indices, gB, gC);
     MUST(cudaDeviceSynchronize());
 }
 
@@ -7957,8 +8173,10 @@ __hoisted_83(uint32_t cols,
              Kuiper_Sparse_Matrix_smatrix__float gA,
              uint32_t *row_indices, float *gB, float *gC)
 {
-    uint32_t m_idx = row_indices[blockIdx.x / ((cols + 511U) / 512U)];
-    uint32_t n_idx = blockIdx.x % ((cols + 511U) / 512U) * 512U;
+    uint32_t m_idx =
+        row_indices[blockIdx.x / (cols / 512U + (cols % 512U != 0U ? 1U : 0U))];
+    uint32_t n_idx =
+        blockIdx.x % (cols / 512U + (cols % 512U != 0U ? 1U : 0U)) * 512U;
     float *elems_tile = (float *)KPR_SHMEM_AT(0U);
     uint32_t *col_ind_tile = (uint32_t *) KPR_SHMEM_AT(1024U);
     uint32_t ri = gA.row_off[m_idx];
@@ -8039,8 +8257,9 @@ Klas_SPMM_g_spmm_f32_512x256x64(uint32_t rows,
     KPR_SHMEM_FITS(2048U);
     MUST(cudaFuncSetAttribute
          (__hoisted_83, cudaFuncAttributeMaxDynamicSharedMemorySize, 2048U));
-    KPR_KCALL(__hoisted_83, rows * ((cols + 511U) / 512U), 64U, 2048U, cols, gA,
-              row_indices, gB, gC);
+    KPR_KCALL(__hoisted_83,
+              rows * (cols / 512U + (cols % 512U != 0U ? 1U : 0U)), 64U, 2048U,
+              cols, gA, row_indices, gB, gC);
     MUST(cudaDeviceSynchronize());
 }
 
@@ -8053,8 +8272,10 @@ __hoisted_84(uint32_t cols,
              Kuiper_Sparse_Matrix_smatrix__float gA,
              uint32_t *row_indices, float *gB, float *gC)
 {
-    uint32_t m_idx = row_indices[blockIdx.x / ((cols + 511U) / 512U)];
-    uint32_t n_idx = blockIdx.x % ((cols + 511U) / 512U) * 512U;
+    uint32_t m_idx =
+        row_indices[blockIdx.x / (cols / 512U + (cols % 512U != 0U ? 1U : 0U))];
+    uint32_t n_idx =
+        blockIdx.x % (cols / 512U + (cols % 512U != 0U ? 1U : 0U)) * 512U;
     float *elems_tile = (float *)KPR_SHMEM_AT(0U);
     uint32_t *col_ind_tile = (uint32_t *) KPR_SHMEM_AT(1024U);
     uint32_t ri = gA.row_off[m_idx];
@@ -8135,8 +8356,9 @@ Klas_SPMM_g_spmm_f32_512x256x128(uint32_t rows,
     KPR_SHMEM_FITS(2048U);
     MUST(cudaFuncSetAttribute
          (__hoisted_84, cudaFuncAttributeMaxDynamicSharedMemorySize, 2048U));
-    KPR_KCALL(__hoisted_84, rows * ((cols + 511U) / 512U), 128U, 2048U, cols,
-              gA, row_indices, gB, gC);
+    KPR_KCALL(__hoisted_84,
+              rows * (cols / 512U + (cols % 512U != 0U ? 1U : 0U)), 128U, 2048U,
+              cols, gA, row_indices, gB, gC);
     MUST(cudaDeviceSynchronize());
 }
 
@@ -8149,8 +8371,10 @@ __hoisted_85(uint32_t cols,
              Kuiper_Sparse_Matrix_smatrix__float gA,
              uint32_t *row_indices, float *gB, float *gC)
 {
-    uint32_t m_idx = row_indices[blockIdx.x / ((cols + 511U) / 512U)];
-    uint32_t n_idx = blockIdx.x % ((cols + 511U) / 512U) * 512U;
+    uint32_t m_idx =
+        row_indices[blockIdx.x / (cols / 512U + (cols % 512U != 0U ? 1U : 0U))];
+    uint32_t n_idx =
+        blockIdx.x % (cols / 512U + (cols % 512U != 0U ? 1U : 0U)) * 512U;
     float *elems_tile = (float *)KPR_SHMEM_AT(0U);
     uint32_t *col_ind_tile = (uint32_t *) KPR_SHMEM_AT(1024U);
     uint32_t ri = gA.row_off[m_idx];
@@ -8231,8 +8455,9 @@ Klas_SPMM_g_spmm_f32_512x256x256(uint32_t rows,
     KPR_SHMEM_FITS(2048U);
     MUST(cudaFuncSetAttribute
          (__hoisted_85, cudaFuncAttributeMaxDynamicSharedMemorySize, 2048U));
-    KPR_KCALL(__hoisted_85, rows * ((cols + 511U) / 512U), 256U, 2048U, cols,
-              gA, row_indices, gB, gC);
+    KPR_KCALL(__hoisted_85,
+              rows * (cols / 512U + (cols % 512U != 0U ? 1U : 0U)), 256U, 2048U,
+              cols, gA, row_indices, gB, gC);
     MUST(cudaDeviceSynchronize());
 }
 
@@ -8245,8 +8470,10 @@ __hoisted_86(uint32_t cols,
              Kuiper_Sparse_Matrix_smatrix__float gA,
              uint32_t *row_indices, float *gB, float *gC)
 {
-    uint32_t m_idx = row_indices[blockIdx.x / ((cols + 511U) / 512U)];
-    uint32_t n_idx = blockIdx.x % ((cols + 511U) / 512U) * 512U;
+    uint32_t m_idx =
+        row_indices[blockIdx.x / (cols / 512U + (cols % 512U != 0U ? 1U : 0U))];
+    uint32_t n_idx =
+        blockIdx.x % (cols / 512U + (cols % 512U != 0U ? 1U : 0U)) * 512U;
     float *elems_tile = (float *)KPR_SHMEM_AT(0U);
     uint32_t *col_ind_tile = (uint32_t *) KPR_SHMEM_AT(2048U);
     uint32_t ri = gA.row_off[m_idx];
@@ -8327,8 +8554,9 @@ Klas_SPMM_g_spmm_f32_512x512x16(uint32_t rows,
     KPR_SHMEM_FITS(4096U);
     MUST(cudaFuncSetAttribute
          (__hoisted_86, cudaFuncAttributeMaxDynamicSharedMemorySize, 4096U));
-    KPR_KCALL(__hoisted_86, rows * ((cols + 511U) / 512U), 16U, 4096U, cols, gA,
-              row_indices, gB, gC);
+    KPR_KCALL(__hoisted_86,
+              rows * (cols / 512U + (cols % 512U != 0U ? 1U : 0U)), 16U, 4096U,
+              cols, gA, row_indices, gB, gC);
     MUST(cudaDeviceSynchronize());
 }
 
@@ -8341,8 +8569,10 @@ __hoisted_87(uint32_t cols,
              Kuiper_Sparse_Matrix_smatrix__float gA,
              uint32_t *row_indices, float *gB, float *gC)
 {
-    uint32_t m_idx = row_indices[blockIdx.x / ((cols + 511U) / 512U)];
-    uint32_t n_idx = blockIdx.x % ((cols + 511U) / 512U) * 512U;
+    uint32_t m_idx =
+        row_indices[blockIdx.x / (cols / 512U + (cols % 512U != 0U ? 1U : 0U))];
+    uint32_t n_idx =
+        blockIdx.x % (cols / 512U + (cols % 512U != 0U ? 1U : 0U)) * 512U;
     float *elems_tile = (float *)KPR_SHMEM_AT(0U);
     uint32_t *col_ind_tile = (uint32_t *) KPR_SHMEM_AT(2048U);
     uint32_t ri = gA.row_off[m_idx];
@@ -8423,8 +8653,9 @@ Klas_SPMM_g_spmm_f32_512x512x32(uint32_t rows,
     KPR_SHMEM_FITS(4096U);
     MUST(cudaFuncSetAttribute
          (__hoisted_87, cudaFuncAttributeMaxDynamicSharedMemorySize, 4096U));
-    KPR_KCALL(__hoisted_87, rows * ((cols + 511U) / 512U), 32U, 4096U, cols, gA,
-              row_indices, gB, gC);
+    KPR_KCALL(__hoisted_87,
+              rows * (cols / 512U + (cols % 512U != 0U ? 1U : 0U)), 32U, 4096U,
+              cols, gA, row_indices, gB, gC);
     MUST(cudaDeviceSynchronize());
 }
 
@@ -8437,8 +8668,10 @@ __hoisted_88(uint32_t cols,
              Kuiper_Sparse_Matrix_smatrix__float gA,
              uint32_t *row_indices, float *gB, float *gC)
 {
-    uint32_t m_idx = row_indices[blockIdx.x / ((cols + 511U) / 512U)];
-    uint32_t n_idx = blockIdx.x % ((cols + 511U) / 512U) * 512U;
+    uint32_t m_idx =
+        row_indices[blockIdx.x / (cols / 512U + (cols % 512U != 0U ? 1U : 0U))];
+    uint32_t n_idx =
+        blockIdx.x % (cols / 512U + (cols % 512U != 0U ? 1U : 0U)) * 512U;
     float *elems_tile = (float *)KPR_SHMEM_AT(0U);
     uint32_t *col_ind_tile = (uint32_t *) KPR_SHMEM_AT(2048U);
     uint32_t ri = gA.row_off[m_idx];
@@ -8519,8 +8752,9 @@ Klas_SPMM_g_spmm_f32_512x512x64(uint32_t rows,
     KPR_SHMEM_FITS(4096U);
     MUST(cudaFuncSetAttribute
          (__hoisted_88, cudaFuncAttributeMaxDynamicSharedMemorySize, 4096U));
-    KPR_KCALL(__hoisted_88, rows * ((cols + 511U) / 512U), 64U, 4096U, cols, gA,
-              row_indices, gB, gC);
+    KPR_KCALL(__hoisted_88,
+              rows * (cols / 512U + (cols % 512U != 0U ? 1U : 0U)), 64U, 4096U,
+              cols, gA, row_indices, gB, gC);
     MUST(cudaDeviceSynchronize());
 }
 
@@ -8533,8 +8767,10 @@ __hoisted_89(uint32_t cols,
              Kuiper_Sparse_Matrix_smatrix__float gA,
              uint32_t *row_indices, float *gB, float *gC)
 {
-    uint32_t m_idx = row_indices[blockIdx.x / ((cols + 511U) / 512U)];
-    uint32_t n_idx = blockIdx.x % ((cols + 511U) / 512U) * 512U;
+    uint32_t m_idx =
+        row_indices[blockIdx.x / (cols / 512U + (cols % 512U != 0U ? 1U : 0U))];
+    uint32_t n_idx =
+        blockIdx.x % (cols / 512U + (cols % 512U != 0U ? 1U : 0U)) * 512U;
     float *elems_tile = (float *)KPR_SHMEM_AT(0U);
     uint32_t *col_ind_tile = (uint32_t *) KPR_SHMEM_AT(2048U);
     uint32_t ri = gA.row_off[m_idx];
@@ -8615,8 +8851,9 @@ Klas_SPMM_g_spmm_f32_512x512x128(uint32_t rows,
     KPR_SHMEM_FITS(4096U);
     MUST(cudaFuncSetAttribute
          (__hoisted_89, cudaFuncAttributeMaxDynamicSharedMemorySize, 4096U));
-    KPR_KCALL(__hoisted_89, rows * ((cols + 511U) / 512U), 128U, 4096U, cols,
-              gA, row_indices, gB, gC);
+    KPR_KCALL(__hoisted_89,
+              rows * (cols / 512U + (cols % 512U != 0U ? 1U : 0U)), 128U, 4096U,
+              cols, gA, row_indices, gB, gC);
     MUST(cudaDeviceSynchronize());
 }
 
@@ -8629,8 +8866,10 @@ __hoisted_90(uint32_t cols,
              Kuiper_Sparse_Matrix_smatrix__float gA,
              uint32_t *row_indices, float *gB, float *gC)
 {
-    uint32_t m_idx = row_indices[blockIdx.x / ((cols + 511U) / 512U)];
-    uint32_t n_idx = blockIdx.x % ((cols + 511U) / 512U) * 512U;
+    uint32_t m_idx =
+        row_indices[blockIdx.x / (cols / 512U + (cols % 512U != 0U ? 1U : 0U))];
+    uint32_t n_idx =
+        blockIdx.x % (cols / 512U + (cols % 512U != 0U ? 1U : 0U)) * 512U;
     float *elems_tile = (float *)KPR_SHMEM_AT(0U);
     uint32_t *col_ind_tile = (uint32_t *) KPR_SHMEM_AT(2048U);
     uint32_t ri = gA.row_off[m_idx];
@@ -8711,8 +8950,9 @@ Klas_SPMM_g_spmm_f32_512x512x256(uint32_t rows,
     KPR_SHMEM_FITS(4096U);
     MUST(cudaFuncSetAttribute
          (__hoisted_90, cudaFuncAttributeMaxDynamicSharedMemorySize, 4096U));
-    KPR_KCALL(__hoisted_90, rows * ((cols + 511U) / 512U), 256U, 4096U, cols,
-              gA, row_indices, gB, gC);
+    KPR_KCALL(__hoisted_90,
+              rows * (cols / 512U + (cols % 512U != 0U ? 1U : 0U)), 256U, 4096U,
+              cols, gA, row_indices, gB, gC);
     MUST(cudaDeviceSynchronize());
 }
 
@@ -8725,8 +8965,10 @@ __hoisted_91(uint32_t cols,
              Kuiper_Sparse_Matrix_smatrix__float gA,
              uint32_t *row_indices, float *gB, float *gC)
 {
-    uint32_t m_idx = row_indices[blockIdx.x / ((cols + 511U) / 512U)];
-    uint32_t n_idx = blockIdx.x % ((cols + 511U) / 512U) * 512U;
+    uint32_t m_idx =
+        row_indices[blockIdx.x / (cols / 512U + (cols % 512U != 0U ? 1U : 0U))];
+    uint32_t n_idx =
+        blockIdx.x % (cols / 512U + (cols % 512U != 0U ? 1U : 0U)) * 512U;
     float *elems_tile = (float *)KPR_SHMEM_AT(0U);
     uint32_t *col_ind_tile = (uint32_t *) KPR_SHMEM_AT(2048U);
     uint32_t ri = gA.row_off[m_idx];
@@ -8806,7 +9048,8 @@ Klas_SPMM_g_spmm_f32_512x512x512(uint32_t rows,
     KPR_SHMEM_FITS(4096U);
     MUST(cudaFuncSetAttribute
          (__hoisted_91, cudaFuncAttributeMaxDynamicSharedMemorySize, 4096U));
-    KPR_KCALL(__hoisted_91, rows * ((cols + 511U) / 512U), 512U, 4096U, cols,
-              gA, row_indices, gB, gC);
+    KPR_KCALL(__hoisted_91,
+              rows * (cols / 512U + (cols % 512U != 0U ? 1U : 0U)), 512U, 4096U,
+              cols, gA, row_indices, gB, gC);
     MUST(cudaDeviceSynchronize());
 }
