src/lib/kuiper/Kuiper.SizeT.fsti
@@ -25,8 +25,8 @@ module SZ = FStar.SizeT
 module U32 = FStar.UInt32
 module U64 = FStar.UInt64
 
-type sz  = FStar.SizeT.t
-type szp = x:sz{FStar.SizeT.v x > 0}
+type sz  = SZ.t
+type szp = x:sz{SZ.v x > 0}
 // Note: making this argument int instead of nat prevents
 // queries about non-negativity from appearing in the well-formedness
 // of types.
@@ -42,9 +42,9 @@ type szpmultiple (k:pos) = x:szp{k /? SZ.v x}
    size_t to uint32_t, which means we should
    NOT assume that a size_t can fit a u64, lest we could get overflow.
 
-   The right thing to do is use FStar.UInt32.t instead of SizeT.t where
+   The right thing to do is use FStar.UInt32.t instead of SZ.t where
    this matters, but this is a pervasive change. *)
-assume SizeTFitsU32 : FStar.SizeT.fits_u32
+assume SizeTFitsU32 : SZ.fits_u32
 
 (* We also assume that those are the ONLY values of size_t that we will
    ever encounter. *)
@@ -54,11 +54,11 @@ val fits_iff_u32 (x:nat)
 
 let fits_ok (x:nat)
   : Lemma (requires my_fits x)
-          (ensures FStar.SizeT.fits x)
-          [SMTPat (FStar.SizeT.fits x)]
+          (ensures SZ.fits x)
+          [SMTPat (SZ.fits x)]
   = assert (x < pow2 32);
     assert_norm (pow2 32 == 0x100000000);
-    FStar.SizeT.fits_u32_implies_fits x
+    SZ.fits_u32_implies_fits x
 
 [@@coercion] unfold let sizet_to_nat  (x: SZ.t)  : GTot nat = SZ.v x
 [@@coercion] unfold let u32_to_nat    (x: U32.t) : GTot nat = U32.v x
@@ -82,12 +82,10 @@ val sizet_and_div_pow2 (x:SZ.t) (y:SZ.t) (n:nat)
 
 inline_for_extraction noextract
 let s_divmod (j:szp) (i:sz) : dm:(sz & szlt j){SZ.fits (dm._1 * j + dm._2)} =
-  let open FStar.SizeT in
-  (i `div` j, i %^ j)
+  (i /^ j, i %^ j)
 
 inline_for_extraction noextract
 let s_undivmod (j:szp) (dm : sz & szlt j {SZ.fits (dm._1 * j + dm._2)}) : sz =
-  let open FStar.SizeT in
   [@@inline_let] let (d, m) = dm in
   d *^ j +^ m
 
@@ -99,11 +97,23 @@ val s_divmod_inv_2 (j:szp) (dm : sz & szlt j {SZ.fits (dm._1 * j + dm._2)})
   : Lemma (s_divmod j (s_undivmod j dm) == dm)
           [SMTPat (s_divmod j (s_undivmod j dm))]
 
+(* Round up division. Extracts to something like
+     (x/y) + (x%y ? 1 : 0) *)
 inline_for_extraction noextract
-val sdivup (x:sz) (y:szp{SZ.fits (x+y)}) : sz
+val sdivup (x : sz) (y : szp) : sz
 
-val lem_sdivup (x:sz) (y:szp{SZ.fits (x+y)})
-  : Lemma (SZ.v (sdivup x y) == divup (SZ.v x) (SZ.v y))
+val lem_sdivup (x : sz) (y : szp)
+  : Lemma (SZ.v (sdivup x y) == divup x y)
+          [SMTPat (sdivup x y)]
+
+(* Also round up division. This version extracts to
+      (x + y - 1) / y
+    but requires the essentially-unfalsifiable precondition that
+    x+y does not overflow. *)
+inline_for_extraction noextract
+val sdivup' (x : sz) (y : szp{SZ.fits (x+y-1)}) : sz
+val lem_sdivup' (x : sz) (y : szp{SZ.fits (x+y-1)})
+  : Lemma (SZ.v (sdivup' x y) == divup x y)
           [SMTPat (sdivup x y)]
 
 inline_for_extraction noextract
@@ -118,5 +128,4 @@ val sdiv_pow2_ok (i:sz{i < 32}) (tid:sz) :
 
 noextract inline_for_extraction
 let smin (a b : sz): sz =
-  let open FStar.SizeT in
   if a <^ b then a else b
